Reorganization of the Separation Logic in MSL. This does not affect users of the Separation Algebras (most of veric for example, or soundness proof in msl/examples/cont/model.v), but it affects the clients of Separation Logic as a "Logic", that is, msl/seplog.v, msl/alg_seplog.v.
The main changes are that there are more axioms for ewand, unfash, and
other things related to subtyping.  Also the Classes in alg_seplog.v have
been reorganized and improved.

Finally, the "cont" case study in msl/examples/cont has been modularized
so that "model.v" uses sep-algs to implement the "logical" interface in
"seplog.v", and then the clients use only the formal logic, not the model.

msl/alg_seplog.v
@@ -38,12 +38,15 @@ Instance algNatDed (T: Type){agT: ageable T} : NatDed (pred T).
  repeat intro. destruct H. apply H0; auto.
  repeat intro. eapply H; eauto. hnf; auto.
  repeat intro. hnf; auto.
+ repeat intro. specialize (H H1 _ H0). hnf in H. auto.
  intros. apply exp_andp1.
+ repeat intro; eapply distrib_orp_andp; auto.
 Defined.
 
 Instance algSepLog (T: Type) {agT: ageable T}{JoinT: Join T}{PermT: Perm_alg T}{SepT: Sep_alg T}{AgeT: Age_alg T} :
       @SepLog (pred T) (algNatDed T).
- apply (mkSepLog _ (algNatDed T) predicates_sl.emp predicates_sl.sepcon predicates_sl.wand).
+ apply (mkSepLog _ (algNatDed T) predicates_sl.emp predicates_sl.sepcon 
+            predicates_sl.wand predicates_sl.ewand).
  apply sepcon_assoc.
  apply sepcon_comm.
  apply @wand_sepcon_adjoint.
@@ -55,6 +58,12 @@ Instance algSepLog (T: Type) {agT: ageable T}{JoinT: Join T}{PermT: Perm_alg T}{
  intros; intro; apply sepcon_derives; auto.
  intros. simpl. apply normalize.sepcon_pure_andp;simpl; auto.
  intros. simpl. apply normalize.pure_sepcon_TT_andp; auto.
+ intros. simpl. apply distrib_orp_sepcon; auto.
+ intros. simpl. apply distrib_sepcon_andp; auto.
+ intros; simpl; apply ewand_sepcon; auto.
+ intros; simpl. apply ewand_TT_sepcon; auto.
+ intros; simpl. intros w [w1 [w2 [? [? ?]]]]. exists w1,w2; repeat split; auto. exists w2; exists w; repeat split; auto.
+  intros; simpl. apply ewand_conflict; auto.
 Defined.
 
 Instance algClassicalSep (T: Type) {agT: ageable T}{JoinT: Join T}{PermT: Perm_alg T}{SepT: Sep_alg T}{CancT: Canc_alg T}{AgeT: Age_alg T}:
@@ -71,6 +80,8 @@ Instance TrivIntuitionistic: IntuitionisticSep Triv.
  destruct H; subst; auto.
 Qed.
 
+
+(*
 Class IndirOps (A: Type) {ND: NatDed A} := mkIndirOps {
   later: A -> A;
   fash : A -> Triv;
@@ -81,67 +92,162 @@ Instance algIndirOps (T: Type) {agT: ageable T}{JoinT: Join T}{PermT: Perm_alg T
          @IndirOps (pred T) (algNatDed T).
  apply (@mkIndirOps (pred T) (algNatDed T) (box laterM) subtypes.fash subtypes.fash').
 Defined.
+*)
 
-Section SL. Import msl.seplog.
-
-Instance TrivIndirOps: IndirOps Triv := 
+ Section SL. Import msl.seplog.
+(*
+ Instance TrivIndirOps: IndirOps Triv := 
      (*Hidden inside a Section, on purpose! *)
-   @algIndirOps nat _ _ _ _ asa_nat. 
+   @algIndirOps nat _ _ _ _ asa_nat.
+*)
+
+
+
+(*
+
+
+
+Lemma subp_e {A}{ND: NatDed A}{IA: Indir A} {P Q : A}: TT |-- P >=> Q -> P |-- Q.
+Admitted.
+
+
+ Lemma subp_i1 {A}{ND: NatDed A}{IA: Indir A}:
+  forall P (Q R: A ), !P && Q |-- R -> P |-- Q >=> R.
+Admitted.
+
+
+Lemma 
+Admitted.
+
+Lemma unfash_sepcon_distrib: 
+        forall {A}{ND: NatDed A}{SA: SepLog A}{IA: Indir A} (P: Triv) (Q R: A),
+               !P && (Q*R) = (!P && Q) * (!P && R).
+Admitted.
+
+Lemma 
+Admitted.
+
+
+ Hint Rewrite @unfash_allp: normalize.
+
+*)
+ 
  
 
 Class Indir (A: Type) {ND: NatDed A} := mkIndir {
-  indir_ops :> IndirOps A;
-  now_later: forall P, P |-- later P;
+  later: A -> A;
+  now_later: forall P: A, P |-- later P;
   later_K: forall P Q, later (P --> Q) |-- later P --> later Q;
-  fash_K: forall P Q, fash (P --> Q) |-- fash P --> fash Q;
   later_derives: forall P Q, P |-- Q -> later P |-- later Q;
-  fash_derives: forall P Q, P |-- Q -> fash P |-- fash Q;
-  later_fash:  forall P, later (fash P) = fash (later P);
   later_andp: forall P Q, later (P && Q) = later P && later Q;
-  fash_andp: forall P Q, fash (P && Q) = fash P && fash Q;
   later_allp: forall T (F: T -> A),  later (allp F) = ALL x:T, later (F x);
   later_exp: forall T (F: T-> A), EX x:T, later (F x) |-- later (exp F);
   later_exp': forall T (any:T) F, later (exp F) = EX x:T, later (F x);
   later_orp: forall P Q, later (P || Q) = later P || later Q;
   later_imp: forall P Q,  later(P --> Q) = later P --> later Q;
-  loeb: forall P,   later P |-- P ->  TT |-- P;
-  subp_allp: forall G B (X Y:B -> A),  (forall x:B, G |-- fash (imp (X x) (Y x))) ->  G |-- fash (imp (allp X) (allp Y));
-  subp_exp: forall G B (X Y:B -> A),  (forall x:B, G |-- fash (imp (X x) (Y x))) ->  G |-- fash (imp (exp X) (exp Y));
-  fash_TT: forall G, G |-- fash TT
+  loeb: forall P,   later P |-- P ->  TT |-- P
 }.
 End SL.
 
 Notation "'|>' e" := (later e) (at level 30, right associativity): logic.
-Notation "'#' e" := (fash e) (at level 30, right associativity): logic.
-Notation "'!' e" := (unfash e) (at level 30, right associativity): logic.
-Notation "P '>=>' Q" := (# (P --> Q)) (at level 55, right associativity) : logic.
-Notation "P '<=>' Q" := (# (P <--> Q)) (at level 57, no associativity) : logic.
 
 Instance algIndir (T: Type) {agT: ageable T}{JoinT: Join T}{PermT: Perm_alg T}{SepT: Sep_alg T}
                 {AgeT: Age_alg T}:
          @Indir (pred T) (algNatDed T).
- apply (mkIndir _ _ (algIndirOps T)); intros; simpl in *.
+ apply (mkIndir _ _ (box laterM)); intros; simpl in *.
  apply @predicates_hered.now_later.
  apply @predicates_hered.axiomK.
- apply @subtypes.fash_K.
  apply @predicates_hered.later_derives; auto.
- apply @subtypes.fash_derives; auto.
- apply @subtypes.later_fash; auto.
  apply @predicates_hered.later_andp.
- apply @subtypes.fash_and.
  apply @predicates_hered.later_allp.
  simpl. intros; apply @box_ex.
   simpl. intros; apply @later_ex; auto.
  apply @later_or.
  apply @predicates_hered.later_imp.
  apply @predicates_hered.loeb; auto.
- apply @subtypes.subp_allp; auto.
- eapply @subtypes.subp_exp; auto. 
- repeat intro; hnf; auto.
 Defined.
+
 
 Instance TrivIndir: Indir Triv := @algIndir nat _ _ _ _ asa_nat.
 
+(* Instance LiftIndirOps (A: Type) (any: A) (B: Type)  {NB: NatDed B} {IB: IndirOps B} : IndirOps (A -> B).
+ apply (@mkIndirOps (A -> B) _ (fun P rho => later (P rho)) (fun P => fash (P any)) 
+            (fun P _ => unfash P)).
+Defined.
+*)
+
+Instance LiftIndir (A: Type) (any: A) (B: Type)  {NB: NatDed B}{IXB: Indir B} :
+         @Indir (A -> B) (LiftNatDed A B).
+ apply (mkIndir _ _ (fun P rho => later (P rho))); intros; simpl in *; intros.
+ apply now_later.
+ apply later_K.
+ apply later_derives; auto.
+ extensionality rho. apply later_andp.
+ simpl; intros. extensionality rho. apply later_allp.
+ simpl; intros. apply later_exp.
+ simpl; intros. extensionality rho. apply later_exp'; auto.
+ simpl; intros. extensionality rho. apply later_orp.
+ simpl; intros. extensionality rho. apply later_imp.
+ simpl; intros. apply loeb; auto.
+Defined.
+
+Section SL2. Import msl.seplog.
+
+Class RecIndir (A: Type) {NA: NatDed A}{IA: Indir A} := mkRecIndir {
+  fash : A -> Triv;
+  unfash : Triv -> A;
+  HORec : forall {X} (f: (X -> A) -> (X -> A)), X -> A;
+  unfash_fash:  forall P: A, unfash (fash P) |-- P;
+  fash_K: forall P Q, fash (P --> Q) |-- fash P --> fash Q;
+  fash_derives: forall P Q, P |-- Q -> fash P |-- fash Q;
+  unfash_derives:  forall P Q,  P |-- Q -> unfash P |-- unfash Q;
+  later_fash:  forall P, later (fash P) = fash (later P);
+  later_unfash:  forall P, later (unfash P) = unfash (later P);
+  fash_andp: forall P Q, fash (P && Q) = fash P && fash Q;
+  unfash_allp:  forall {B} (P: B -> Triv), unfash (allp P) = ALL x:B, unfash (P x);  subp_allp: forall G B (X Y:B -> A),  (forall x:B, G |-- fash (imp (X x) (Y x))) ->  G |-- fash (imp (allp X) (allp Y));
+  subp_exp: forall G B (X Y:B -> A),  (forall x:B, G |-- fash (imp (X x) (Y x))) ->  G |-- fash (imp (exp X) (exp Y)); 
+  subp_e: forall (P Q : A), TT |-- fash (P --> Q) -> P |-- Q;
+  subp_i1: forall P (Q R: A), unfash P && Q |-- R -> P |-- fash (Q --> R);
+ fash_TT: forall G, G |-- fash TT;
+  HOcontractive: forall {X: Type} (f: (X -> A) -> (X -> A)), Prop :=
+         fun {X} f => forall P Q,  (ALL x:X, later (fash (P x <--> Q x))) |-- (ALL x:X, fash (f P x <--> f Q x)); 
+  HORec_fold_unfold : forall X (f: (X -> A) -> (X -> A)) (H: HOcontractive f), HORec f = f (HORec f)
+}.
+
+Definition HOnonexpansive {A}{NA: NatDed A}{IA: Indir A}{RA: RecIndir A}
+        {X: Type} (f: (X -> A) -> (X -> A)) :=
+         forall P Q: X -> A,  (ALL x:X, fash (P x <--> Q x)) |-- (ALL x:X, fash (f P x <--> f Q x)).
+End SL2.
+
+
+Notation "'#' e" := (fash e) (at level 30, right associativity): logic.
+Notation "'!' e" := (unfash e) (at level 30, right associativity): logic.
+Notation "P '>=>' Q" := (# (P --> Q)) (at level 55, right associativity) : logic.
+Notation "P '<=>' Q" := (# (P <--> Q)) (at level 57, no associativity) : logic.
+
+Definition algRecIndir (T: Type) {agT: ageable T}{JoinT: Join T}{PermT: Perm_alg T}{SepT: Sep_alg T}{AgeT: Age_alg T} :
+         @RecIndir (pred T) (algNatDed T) (algIndir T).
+ apply (mkRecIndir _ _ _ subtypes.fash subtypes.fash' HoRec.HORec); intros; simpl.
+ repeat intro. do 3 red in H. apply H; auto.
+ apply @subtypes.fash_K.
+ apply @subtypes.fash_derives; auto.
+ intros ? ?. do 3 red in H0. apply H in H0. apply H0.
+ apply @subtypes.later_fash; auto.
+ apply @subtypes.later_fash'.
+ apply @subtypes.fash_and.
+ apply pred_ext; repeat intro; do 3 red in H; apply (H b); auto.
+ apply @subtypes.subp_allp; auto.
+ eapply @subtypes.subp_exp; auto.
+ eapply @subtypes.subp_e; eauto.
+ eapply @subtypes.subp_i1; eauto. 
+ repeat intro; hnf; auto.
+ intros. apply HoRec.HORec_fold_unfold; auto.
+Defined.
+
+Instance TrivRecIndir: RecIndir Triv := algRecIndir nat.
+
+
+Section SL3. Import msl.seplog.
 
 Lemma fash_triv: forall P: Triv, fash P = P.
 Proof.
@@ -152,60 +258,8 @@ Proof.
  apply nec_nat. auto.
 Qed.
 
-
-Instance LiftIndirOps (A: Type) (any: A) (B: Type)  {NB: NatDed B} {IB: IndirOps B} : IndirOps (A -> B).
- apply (@mkIndirOps (A -> B) _ (fun P rho => later (P rho)) (fun P => fash (P any)) 
-            (fun P rho => unfash P)).
-Defined.
-
-Instance LiftIndir (A: Type) (any: A) (B: Type)  {NB: NatDed B}{IXB: Indir B} :
-         @Indir (A -> B) (LiftNatDed A B).
- apply (mkIndir _ _ (LiftIndirOps A any B)); intros; simpl in *; intros.
- apply now_later.
- apply later_K.
- apply @fash_K; auto.
- apply later_derives; auto.
- apply fash_derives; auto.
- rewrite <- later_fash. simpl. auto.
- extensionality rho. apply later_andp.
- simpl; intros. apply @fash_andp; auto.
- simpl; intros. extensionality rho. apply later_allp.
- simpl; intros. apply later_exp.
- simpl; intros. extensionality rho. apply later_exp'; auto.
- simpl; intros. extensionality rho. apply later_orp.
- simpl; intros. extensionality rho. apply later_imp.
- simpl; intros. apply loeb; auto.
- apply subp_allp; auto.
- apply subp_exp; auto.
- apply fash_TT.
-Defined.
-
-Section SL2. Import msl.seplog.
-
-Class RecIndir (A: Type) {NA: NatDed A}{IA: Indir A} := mkRecIndir {
-  HORec : forall {X} (f: (X -> A) -> (X -> A)), X -> A;
-  HOcontractive: forall {X: Type} (f: (X -> A) -> (X -> A)), Prop :=
-         fun {X} f => forall P Q,  (ALL x:X, later (fash (P x <--> Q x))) |-- (ALL x:X, fash (f P x <--> f Q x)); 
-  HORec_fold_unfold : forall X (f: (X -> A) -> (X -> A)) (H: HOcontractive f), HORec f = f (HORec f)
-}.
-
-Definition HOnonexpansive {A}{NA: NatDed A}{IA: Indir A}
-        {X: Type} (f: (X -> A) -> (X -> A)) :=
-         forall P Q,  (ALL x:X, fash (P x <--> Q x)) |-- (ALL x:X, fash (f P x <--> f Q x)).
-End SL2.
-
-Definition algRecIndir (T: Type) {agT: ageable T}{JoinT: Join T}{PermT: Perm_alg T}{SepT: Sep_alg T}{AgeT: Age_alg T} :
-         @RecIndir (pred T) (algNatDed T) (algIndir T).
- apply (mkRecIndir _ _ _ HoRec.HORec).
- intros. apply HoRec.HORec_fold_unfold; auto.
-Defined.
-
-Instance TrivRecIndir: RecIndir Triv := algRecIndir nat.
-
-Section SL3. Import msl.seplog.
 Class SepIndir (A: Type) {NA: NatDed A}{SA: SepLog A}{IA: Indir A} := mkSepIndir {
-  later_sepcon: forall P Q, |> (P * Q) = |>P * |>Q;
-  sub_sepcon': forall P P' Q Q': A, (P >=> P') && (Q >=> Q') |-- (P * Q) >=> (P' * Q')
+  later_sepcon: forall P Q, |> (P * Q) = |>P * |>Q
 }.
 End SL3.
 
@@ -214,6 +268,26 @@ Instance algSepIndir (T: Type) {agT: ageable T}{JoinT: Join T}{PermT: Perm_alg T
  apply mkSepIndir.
  simpl.
  apply @predicates_sl.later_sepcon; auto.
+Qed.
+
+Instance LiftSepIndir  (A: Type) (any: A) (B: Type)  {NB: NatDed B} {SB: SepLog B}{IB: Indir B}{SIB: SepIndir B} : 
+     @SepIndir (A -> B) (LiftNatDed A B) (LiftSepLog A B) (LiftIndir A any B).
+ constructor.
+ intros; simpl. extensionality rho.  apply later_sepcon.
+Qed.
+
+Section SL4. Import msl.seplog.
+Class SepRec  (A: Type) {NA: NatDed A}{SA: SepLog A}{IA: Indir A}{RA: RecIndir A} := mkSepRec {
+  unfash_sepcon_distrib: forall (P: Triv) (Q R: A),
+                 andp (unfash P) (sepcon Q R) = sepcon (andp (unfash P) Q) (andp (unfash P) R); 
+  sub_sepcon': forall P P' Q Q': A, (P >=> P') && (Q >=> Q') |-- (P * Q) >=> (P' * Q')
+}.
+End SL4.
+
+Instance algSepRec (T: Type) {agT: ageable T}{JoinT: Join T}{PermT: Perm_alg T}{SepT: Sep_alg T}{AgeT: Age_alg T} :
+         @SepRec (pred T) (algNatDed T) (algSepLog T) (algIndir T)(algRecIndir T).
+constructor.
+ intros; simpl. apply subtypes_sl.unfash_sepcon_distrib.
 
   repeat intro. destruct H.
   destruct H2 as [w1 [w2 [? [? ?]]]].
@@ -228,12 +302,3 @@ Instance algSepIndir (T: Type) {agT: ageable T}{JoinT: Join T}{PermT: Perm_alg T
   apply comparable_fashionR. eapply join_sub_comparable; eauto.
  apply necR_level in H1. omega.
 Qed.
-
-Instance LiftSepIndir  (A: Type) (any: A) (B: Type)  {NB: NatDed B} {SB: SepLog B}{IB: Indir B}{SIB: SepIndir B} : 
-     @SepIndir (A -> B) (LiftNatDed A B) (LiftSepLog A B) (LiftIndir A any B).
- constructor.
- intros; simpl. extensionality rho.  apply later_sepcon.
- intros; simpl. intros rho ?. apply sub_sepcon'. auto.
-Qed.
-
-
