msl/examples/cont/language.v
@@ -1,5 +1,6 @@
 Require Import Arith.
 Require Import List.
+Require Import msl.base.
 Require Import msl.eq_dec.
 
 Definition table (A B : Type) := list (A*B).
@@ -47,7 +48,7 @@ Notation " a '.+' n " := (Offset a n) (at level 87, no associativity).
 
 Inductive control := 
 | Assign: expr -> expr -> control -> control
-| If: expr -> control -> control -> control
+| IfThenElse: expr -> control -> control -> control
 | Go: expr -> list expr -> control.
 
 Definition program := table adr (list var * control).
@@ -107,7 +108,7 @@ Definition step (p: program) (sk: state) : option state :=
                            do1 p <- expr_get stk hp x;
                            Some ((stk, heap_set p v hp), c)
  | (_, Assign _ y c) => None
- | ((stk,hp), If x c1 c2) => 
+ | ((stk,hp), IfThenElse x c1 c2) => 
                            do1 v <- expr_get stk hp x;
                            Some (if eq_dec v 0 then ((stk,hp), c2) else ((stk,hp), c1))
  | ((stk, hp), Go x ys) =>   
@@ -134,6 +135,228 @@ Definition run (p: program) (n: nat) : option state :=
     stepN p (nil, initial_heap p, Go (Const 0) (Const (boundary p) :: nil)) n.
 
 Notation "'Do' x ':=' v ';' c" := (Assign x v c) (at level 200, x at level 1, v at level 90, c at level 200).
-Notation "'If' x 'Then' c1 'Else' c2" := (If x c1 c2)  (at level 200, x at level 90, c1 at level 200, c2 at level 200).
+Notation "'If' x 'Then' c1 'Else' c2" := (IfThenElse x c1 c2)  (at level 200, x at level 90, c1 at level 200, c2 at level 200).
 
 Definition safe (p: program) : Prop :=  forall n, exists sk', run p n = Some sk'.
+
+(* LOCAL VARIABLE ENVIRONMENTS *)
+
+Definition env := var -> adr.
+
+Definition env_set (f: env) (x: var) (y: adr) :=
+   fun i => if eq_dec i x then y else f i.
+
+Lemma env_gss : forall s x y, env_set s x y x = y.
+Proof. unfold env_set; intros.  destruct (eq_dec x x); auto. congruence.
+Qed.
+Lemma env_gso: forall s x y z, x<>z -> env_set s x y z = s z.
+Proof. unfold env_set; intros. destruct (eq_dec z x); auto. congruence.
+Qed.
+
+Definition locals2env (s: locals) : env := 
+   fun x => match table_get s x with Some a => a | None => 0 end.
+
+Fixpoint eval (e: expr) : env -> adr :=
+ fun s =>
+ match e with
+ | Const n => n
+ | Var x => s x
+ | Offset e n => n + eval e s
+ | Mem e => 0
+ end.
+
+Definition eval_list (xs: list expr) : env -> (list adr) := fun s => map (fun e => eval e s) xs.
+
+Lemma offset_zero:  forall a, eval (a .+ 0) = eval a.
+Proof. intros. extensionality s; simpl; destruct (eval a s); simpl; f_equal; auto.
+Qed.
+
+Lemma offset_offset: forall a n m, 
+  eval ((a .+ n) .+ m) = eval (a .+ (n+m)).
+Proof.
+ intros.
+ extensionality s. simpl.
+Transparent adr. unfold adr; omega.
+Opaque adr.
+Qed.
+
+Definition arguments (vars: list var) (vl: list adr) : env :=
+      locals2env (mk_locals vars vl).
+Opaque arguments.
+
+
+Lemma locals2env_table_set: 
+  forall x y s, locals2env (table_set x y s) = env_set (locals2env s) x y.
+Proof. intros; extensionality i. unfold locals2env, env_set, table_set.
+  simpl. destruct (eq_dec i x); auto.
+Qed.
+
+Definition subst{A} (x: var) (v: adr) (P: env -> A) : env -> A :=
+   fun s => P (env_set s x v).
+
+
+(* TYPE-CHECKING OF LOCAL VARIABLES *)
+Require Import msl.Coqlib2.
+
+Require ListSet.
+Definition varset : Type := ListSet.set var.
+Definition vs_mem: var -> varset -> bool := ListSet.set_mem EqDec_var.
+Definition vs_add: var -> varset -> varset := ListSet.set_add EqDec_var.
+
+Definition varcompat (vars: varset) (s: locals) :=
+   forall i, vs_mem i vars = true -> table_get s i <> None.
+
+Fixpoint expcheck (vars: varset) (e: expr) :=
+  match e with
+  | Const _ => true
+  | Var v => vs_mem v vars
+  | Offset e n => expcheck vars e
+  | Mem _ => false
+  end.
+
+Fixpoint typecheck (vars: varset) (c: control) : bool :=
+ match c with 
+  | Assign (Var v) (Mem e) c' => andb (expcheck vars e)
+                                         (typecheck (vs_add v vars) c')
+  | Assign (Var v) e c' => andb (expcheck vars e)
+                                         (typecheck (vs_add v vars) c')
+  | Assign (Mem e1) e2 c' => andb (andb (expcheck vars e1)  (expcheck vars e2))
+                                         (typecheck vars c')
+  | IfThenElse e c1 c2 => andb (expcheck vars e) 
+                                            (andb (typecheck vars c1) (typecheck vars c2))
+  | Go e el => andb (expcheck vars e)  (forallb (expcheck vars) el)
+  | _ => false
+  end.
+
+Lemma eval_expr_get:
+  forall vars s h e, 
+              expcheck vars e = true ->
+              varcompat vars s ->
+              expr_get s h e = Some (eval e (locals2env s)).
+Proof. induction e; simpl; auto; intros.
+  apply H0 in H. unfold locals2env. 
+ destruct (table_get s v); auto. congruence.
+  specialize (IHe H H0). rewrite IHe. simpl.   f_equal; omega. 
+  inv H.
+Qed.
+
+Lemma eval_expr_get_list:
+  forall vars s h el, 
+              forallb (expcheck vars) el = true ->
+              varcompat vars s ->
+              get_list s h el = Some (eval_list el (locals2env s)).
+Proof. induction el; simpl; auto; intros.
+ rewrite andb_true_iff in H; destruct H.
+  rewrite (eval_expr_get vars s h a); auto. simpl.
+  rewrite (IHel H1 H0); auto.
+Qed.
+
+Lemma varcompat_add:
+  forall x vars z s, varcompat vars s -> varcompat (vs_add x vars) (table_set x z s).
+Proof.
+ intros. intros i ?. specialize (H i).
+ unfold vs_mem, vs_add in *.
+ apply ListSet.set_mem_correct1 in H0.
+ destruct (eq_dec i x). 
+ subst. rewrite table_gss. congruence.
+ rewrite table_gso; auto. apply H.
+ apply ListSet.set_add_elim2 in H0; auto.
+ apply ListSet.set_mem_correct2; auto.
+Qed.
+
+Lemma varcompat_mk_locals:
+  forall xl vl, length xl <= length vl -> varcompat xl (mk_locals xl vl).
+Proof. 
+ unfold varcompat, vs_mem, mk_locals. intros.
+ revert vl H H0; induction xl; destruct vl; intros.
+ apply ListSet.set_mem_correct1 in H0. inv H0.
+ apply ListSet.set_mem_correct1 in H0. inv H0.
+ inv H. simpl in H.
+ specialize (IHxl vl). spec IHxl ; [ omega |].
+ apply ListSet.set_mem_correct1 in H0. simpl in H0. destruct H0.
+ subst. simpl.
+destruct (eq_dec i i); auto. congruence.
+ simpl. destruct (eq_dec i a). congruence.
+ apply IHxl. 
+ apply ListSet.set_mem_correct2. auto.
+Qed.
+
+Definition inlist {A: Type}{EA: EqDec A} (x: A) (vl: list A) : bool :=
+   existsb (fun y => if eq_dec x y then true else false) vl.
+
+Lemma inlist_notIn {A: Type}{EA: EqDec A}:
+  forall (x: A) (vl: list A), inlist x vl = false -> ~ In x vl.
+Proof.
+  induction vl; simpl; intros; intuition.
+  subst. destruct (eq_dec x x); auto. inv H.
+  destruct (eq_dec x a). inv H. simpl in H. auto.
+Qed. 
+
+Fixpoint list_nodups {A: Type}{EA: EqDec A} (vl: list A) : bool :=
+  match vl with
+  | nil => true
+  | x::xl => andb (negb (inlist x xl)) (list_nodups xl)
+  end.
+
+Inductive list_norepet {A: Type} : list A -> Prop :=
+  | list_norepet_nil:
+      list_norepet nil
+  | list_norepet_cons:
+      forall hd tl,
+      ~(In hd tl) -> list_norepet tl -> list_norepet (hd :: tl).
+
+Lemma nodups_norepet  {A: Type}{EA: EqDec A} :
+    forall l, list_nodups l = true -> list_norepet l.
+Proof. induction l; intros.
+  constructor.
+  simpl in H. apply andb_true_iff in H. 
+  destruct H.
+  constructor; auto.
+  apply inlist_notIn. destruct (inlist a l); auto; inv H.
+Qed.
+
+(* SAFE FOR N STEPS *)
+
+Definition safeN (p: program) (sk: state) (n: nat) : Prop :=
+   exists sk', stepN p sk n = Some sk'.
+
+Lemma stepN_plus: forall p sk1 n1 n2 sk3,
+   stepN p sk1 (n1+n2) = Some sk3 <->
+   (exists sk2, stepN p sk1 n1 = Some sk2 /\ stepN p sk2 n2 = Some sk3).
+Proof.
+ induction n1; intros. 
+ simpl; split; eauto. intros [sk2 [? ?]]. inv H; auto.
+ replace (S n1 + n2) with (n1 + S n2) by omega.
+ rewrite (IHn1 (S n2) sk3).
+ split; intros [sk2 [? ?]].
+ simpl in H0; invSome.
+ exists s. split; auto.
+ replace (S n1) with (n1 + 1) by omega.
+ rewrite (IHn1 1). exists sk2; split; simpl; auto. rewrite H0; auto.
+ replace (S n1) with (n1 + 1) in H by omega.
+ rewrite (IHn1 1) in H. destruct H as [sk4 [? ?]].
+ exists sk4; split; simpl; auto. simpl in H1.  invSome. auto. 
+Qed.
+
+Lemma safeN_less: forall p sk n1 n2, n1 <= n2 -> safeN p sk n2 -> safeN p sk n1.
+Proof.
+ intros.
+ assert (n2 = n1 + (n2-n1)) by omega.
+ rewrite H1 in H,H0.
+ forget (n2-n1) as k.
+ clear n2 H1 H.
+ destruct H0 as [sk' ?].
+ rewrite stepN_plus in H.
+ destruct H as [sk2 [? ?]]; exists sk2; auto.
+Qed.
+
+Lemma safeN_step:
+  forall p sk sk' n, step p sk = Some sk' -> (safeN p sk (S n) <-> safeN p sk' n).
+Proof.
+  unfold safeN; intros.
+  split; intros [sk2 ?].
+  exists sk2.
+ simpl in H0. rewrite H in H0. auto.
+  exists sk2; simpl.  rewrite H; auto.
+Qed.
+
