msl/examples/cont/lseg.v
@@ -1,11 +1,27 @@
 Require Import msl.examples.cont.language.
-Require Import msl.examples.cont.sep_base.
-Require Import msl.msl_standard.
+Require Import msl.base.
+Require Import msl.seplog.
+Require Import msl.alg_seplog.
+Require Import msl.examples.cont.seplog.
 Require Import msl.Coqlib2.
+Require Import msl.log_normalize.
+Require Import msl.eq_dec.
 
-Local Open Scope pred.
+Local Open Scope logic.
 
-Definition next e1 e2: pred rmap := !! (e1 > 0) && mapsto e1 e2.
+
+Declare Module Semax : SEMAX.  
+ (* Remark:  "Declare Module" is a hack.
+  We want to emphasize that the client proofs (in lseg.v, client_lemmas.v,
+   and sample_program.v) can be done independently of the 
+   model.v that implements the Module Semax.  The correct way to do
+   this in Coq is to use a parameterized Module (that is, a Functor),
+   which is not difficult but in this example we wanted to avoid
+   a heavyweight use of the module system. *)
+
+Import Semax.
+
+Definition next e1 e2: mpred := !! (e1 > 0) && mapsto e1 e2.
 
 Lemma next_gt_0: 
   forall x y, next x y = !! (x>0) && next x y.
@@ -16,163 +32,45 @@ Qed.
 
 Lemma next_neq_0: forall y, next 0 y |-- FF.   (* W1 *)
 Proof.
- intros. rewrite next_gt_0. apply prop_andp_left. intro. inv H.
+ intros. rewrite next_gt_0. normalize. inv H.
 Qed.
 
-Definition listcons' (R: (adr * adr) -> pred rmap) (lp: adr * adr) : pred rmap :=
-      !! (fst lp <> snd lp) && Ex tail:adr, next (fst lp) tail * |> R (tail, snd lp).
+Definition listcons' (R: (adr * adr) -> mpred) (lp: adr * adr) : mpred :=
+      !! (fst lp <> snd lp) && EX tail:adr, next (fst lp) tail * |> R (tail, snd lp).
 
-Definition listempty (lp: adr*adr) : pred rmap :=
+Definition listempty (lp: adr*adr) : mpred :=
              !! (fst lp = snd lp) && emp.
  
-Definition listrep' (R: adr*adr -> pred rmap) (lp: adr*adr) : pred rmap :=
+Definition listrep' (R: adr*adr -> mpred) (lp: adr*adr) : mpred :=
         listcons' R lp || listempty lp.
 
-Definition listrep : adr*adr -> pred rmap := HORec listrep'.
+Definition listrep : adr*adr -> mpred := HORec listrep'.
 
-Definition lseg (e1 e2: adr) : pred rmap := listrep (e1,e2).
-
-
-Lemma orp_HOcontractive {A}{agA: ageable A}: forall X (P Q: (X -> pred A) -> (X -> pred A)),
-       HOcontractive P -> HOcontractive Q -> HOcontractive (fun R x => P R x || Q R x).
-Proof.
- intros.
- intros F G n H2 x y Hy.
- specialize (H F G n H2 x y Hy). specialize (H0 F G n H2 x y Hy).
- destruct H, H0.
- split; (intros z Hz [?|?]; [left|right]); auto.
-Qed.
-Lemma andp_HOcontractive {A}{agA: ageable A}: forall X (P Q: (X -> pred A) -> (X -> pred A)),
-       HOcontractive P -> HOcontractive Q -> HOcontractive (fun R x => P R x && Q R x).
-Proof.
- intros.
- intros F G n H2 x y Hy.
- specialize (H F G n H2 x y Hy). specialize (H0 F G n H2 x y Hy).
- destruct H, H0.
- split; (intros z Hz [? ?]); split; auto.
-Qed.
-Lemma sepcon_HOcontractive {A} {JA: Join A}{PA: Perm_alg A}{SA: Sep_alg A}{AG: ageable A}{XA: Age_alg A}{NA: natty A}: forall X (P Q: (X -> pred A) -> (X -> pred A)),
-       HOcontractive P -> HOcontractive Q -> HOcontractive (fun R x => P R x * Q R x).
-Proof.
- intros.
- unfold HOcontractive in *|-.
- apply prove_HOcontractive; intros F G ?.
- specialize (H F G). specialize (H0 F G).
- apply subp_sepcon.
- eapply derives_trans.
- apply allp_derives; intro. rewrite <- eq_later. apply derives_refl.
- eapply derives_trans; [ apply H | ].
- apply allp_left with x.
- apply fash_derives. apply andp_left1. auto.
- eapply derives_trans.
- apply allp_derives; intro. rewrite <- eq_later. apply derives_refl.
- eapply derives_trans; [ apply H0 | ].
- apply allp_left with x.
- apply fash_derives. apply andp_left1. auto.
-Qed.
-
-Lemma const_HOcontractive{A}{agA: ageable A}: forall X (P : X -> pred A), HOcontractive (fun _ => P).
-Proof.
- intros.
- apply prove_HOcontractive. intros. apply sub_refl.
-Qed.
-
-Lemma exp_HOcontractive {A}{agA: ageable A}{NA: natty A}:
-  forall X Y (G: Y -> X -> X) (F: Y -> X -> pred A -> pred A),
-   (forall y x, contractive (F y x)) ->
-   HOcontractive (fun (R: X -> pred A) (x: X) => Ex y: Y, F y x (R (G y x))).
-Proof.
- intros.
- apply prove_HOcontractive; intros.
- apply sub_exp; intro y.
- specialize (H y x (P (G y x)) (Q (G y x))).
- eapply derives_trans; [ | apply equ_sub; apply H].
- rewrite eq_later.
- apply allp_left with (G y x). auto.
-Qed.
-Lemma const_contractive {A}{agA: ageable A}: forall P : pred A, contractive (fun _ => P).
-Proof.
- intros.
- apply prove_contractive. intros. apply sub_refl.
-Qed.
-Lemma later_contractive' {A} `{natty A} : contractive (box laterM).
-Proof.
-  unfold contractive; intros.
-  apply sub_equ.
-  rewrite <- sub_later.
-  apply box_positive; auto.
-  apply equ_sub; auto.
-  rewrite <- sub_later.
-  apply box_positive; auto.
-  apply equ_sub2; auto.
-Qed.
+Definition lseg (e1 e2: adr) : mpred := listrep (e1,e2).
 
 Lemma lseg_unfold: forall e1 e2, 
-   (lseg e1 e2 = (!! (e1<> e2)  && Ex tail:adr, next e1 tail * |> lseg tail e2)
-                        || (!! (e1=e2) && emp))%pred.
+   (lseg e1 e2 = (!! (e1<> e2)  && EX tail:adr, next e1 tail * |> lseg tail e2)
+                        || (!! (e1=e2) && emp)).
 Proof.
  intros.
  unfold lseg. unfold listrep at 1.
  rewrite HORec_fold_unfold. reflexivity.
-
- apply prove_HOcontractive. intros. unfold listrep', listcons'.
-
- unfold listrep'.
- apply orp_HOcontractive.
- unfold listcons'.
- apply andp_HOcontractive.
- apply const_HOcontractive.
- apply exp_HOcontractive with (G:= fun y x => (y, snd x))
-                   (F := fun tail x P => next (fst x) tail * |> P);  
-   intros.
- apply sepcon_contractive.
- apply const_contractive.
- apply later_contractive'.
- apply const_HOcontractive.
-Qed.
-
-Lemma exists_contractive {A} `{ageable A} : forall B (X : pred A -> B -> pred A),
-  (forall x, (contractive (fun y => X y x))) ->
-  contractive (fun x => (exp (X x))).
-Proof.
-  unfold contractive; intros.
-  apply sub_equ; apply sub_exp; intros.
-  apply equ_sub; auto.
-  apply equ_sub2; auto.
-Qed.
-
-
-Print const_HOcontractive.
-
-
-Print Hint.
- intros ? ? ?.
- -> (X -> pred A)),
-Search HOcontractive.
-
-Print Hint.
- auto with contractive.
-
-
-
-
- auto 50 with contractive.
- auto 50 with contractive.
- do 3 red in H0.
+ unfold listrep', listcons'.
+ apply prove_HOcontractive. auto 50 with contractive typeclass_instances.
 Qed.
 
 Lemma lseg_neq: forall p q: adr, p<>q -> 
-        lseg p q = Ex y:adr, next p y *  |> lseg y q.
+        lseg p q = EX y:adr, next p y *  |> lseg y q.
 Proof.
  intros.
  apply pred_ext.
  rewrite lseg_unfold at 1.
  apply orp_left.
- apply andp_left2. apply exp_derives; intro y.
- apply sepcon_derives; auto.
- apply prop_andp_left; contradiction.
+ normalize. apply exp_right with tail. auto.
+ normalize.
+ normalize; intro y.
  rewrite (lseg_unfold p q). apply orp_right1.
- apply prop_andp_right; auto.
+ normalize. apply exp_right with y. normalize.
 Qed.
 
 Lemma lseg_eq: forall a, lseg a a = emp.
@@ -180,9 +78,9 @@ Proof.
  intros. rewrite lseg_unfold.
  apply pred_ext.
  apply orp_left.
- apply prop_andp_left; congruence.
- apply prop_andp_left; auto.
- apply orp_right2. apply prop_andp_right; auto. 
+ normalize.  congruence.
+ normalize.
+ apply orp_right2. normalize.
 Qed.
 
 Lemma lseg_cons: (* U2 *)
@@ -191,10 +89,10 @@ Proof.
  intros.
  pattern lseg at 1; rewrite lseg_unfold.
  apply orp_right1.
- apply prop_andp_right; auto.
+ normalize.
  apply exp_right with y.
+ normalize.
  apply sepcon_derives; auto.
- unfold lseg.
  apply now_later.
 Qed.
 
@@ -206,10 +104,8 @@ Proof.
  apply andp_left2.
  apply exp_left; intro v.
  rewrite next_gt_0.
- rewrite sepcon_andp_prop1.
- apply prop_andp_left; intro. inv H.
- apply andp_left1.
- intros w ?; hnf in *; auto.
+ normalize. inv H.
+ normalize.
 Qed.
 
 Lemma next_lseg:  (* U1 *)
@@ -222,17 +118,6 @@ Proof.
 Qed.
 
 
-Lemma mapsto_conflict:
-   forall a b c, mapsto a b  *  mapsto a c |-- FF.
-  Proof.
-    intros. intros w  [w1 [w2 [? [? ?]]]]; hnf.
-    specialize (H0 a). specialize (H1 a).
-    rewrite if_true in * by auto.
-    apply (resource_at_join _ _ _ a) in H.
-    rewrite H0 in H; rewrite H1 in H; inv H.
-    pfullshare_join.
- Qed.
-
 Lemma next_conflict:  (*  W3 *)
    forall x y y', next x y * next x y' |-- FF.
 Proof.
@@ -241,37 +126,24 @@ Proof.
   apply sepcon_derives; apply andp_left2; auto.
 Qed.
 
-Lemma not_prop_right: forall P (Q: Prop), (Q -> P |-- FF) -> P |-- !! (not Q).
- Proof. intros. intros w ? ?. specialize (H H1 w H0); auto. 
-  Qed.
-
  Lemma next_conflict_list: (* W4 *)
      forall x y z, next x y * lseg z 0 |-- !!(x<>z).
  Proof.
    intros.
-   unfold next.
+  apply not_prop_right. intro; subst z.
    rewrite lseg_unfold.
   rewrite sepcon_comm.
   rewrite distrib_orp_sepcon.
   apply orp_left.
-  repeat rewrite sepcon_andp_prop1. 
-  apply andp_left2.
-  rewrite exp_sepcon1.
-  apply exp_left; intro v. 
-  rewrite sepcon_comm.
+  normalize.
+  rewrite sepcon_comm. 
   rewrite <- sepcon_assoc.
-  apply @derives_trans with (!! (x<>z) && TT * TT).
-  apply sepcon_derives; auto.
-  apply andp_right; auto. 
-  apply not_prop_right; intros; subst; apply next_conflict.
-  rewrite sepcon_andp_prop1.
-  apply andp_left1; auto.
-  rewrite sepcon_andp_prop1. rewrite emp_sepcon.
-  apply prop_andp_left; intro.
-  subst.
-  unfold next.
-  apply prop_andp_left; intro.
-  intros ? ?; hnf; omega.
+  eapply derives_trans with (FF * TT).
+  apply sepcon_derives; normalize.
+  apply next_conflict.
+  normalize.
+  unfold next;   normalize.
+  inv H.
 Qed.
 
 Lemma lseg_W5: forall x y z,   (* W5 *)
@@ -291,153 +163,143 @@ Proof.
   rewrite (sepcon_comm (|> _)).
   repeat rewrite <- sepcon_assoc. rewrite sepcon_assoc.
   eapply derives_trans. apply sepcon_derives. apply next_conflict. apply derives_refl.
-  rewrite FF_sepcon. auto.
+  rewrite FF_sepcon. normalize.
 Qed.
 
-(* This lemma is not currently used, 
-    but it might be useful in a different proof of lseg_cons_in_mapsto_context, etc. *)
-Lemma sepcon_andp_fash'1 {A}{JA: Join A}{PA: Perm_alg A}{agA: ageable A}{AgeA: Age_alg A}:  
-    forall (P: pred nat) (Q R : pred A),  fash' P && Q * R = fash' P && (Q * R).
- Proof.
-  intros. apply pred_ext; intros w ?.
-   destruct H as [w1 [w2 [? [? ?]]]].
-   destruct H0. split.
-   hnf in H0|-*. replace (level w) with (level w1); auto.
-   apply join_level in H; intuition.
-    exists w1; exists w2; split3; auto.
-   destruct H.
-   destruct H0 as [w1 [w2 [? [? ?]]]]; exists w1; exists w2; split3; auto.
-   split; auto.
-   hnf in H|-*. replace (level w1) with (level w); auto.
-   apply join_level in H0; intuition.
+Lemma unfash_andp_distrib: 
+        forall {A}{ND: NatDed A}{IA: Indir A}{RA: RecIndir A} (P: Triv) (Q R: A),
+               !P && (Q && R) = (!P && Q) && (!P && R).
+Proof.
+intros. apply pred_ext;  repeat apply andp_right.
+apply andp_left1; auto. apply andp_left2; apply andp_left1; auto.
+apply andp_left1; auto. apply andp_left2; apply andp_left2; auto.
+apply andp_left1; auto. apply andp_left1; auto.
+apply andp_left1; auto. apply andp_left2; auto.
+apply andp_left2; auto. apply andp_left2; auto.
 Qed.
+
 
 Lemma lseg_cons_in_next_context:   (*  U4 *)
     forall x y z v, lseg x y * next y z * next z v |-- lseg x z * next z v.
 Proof.
   intros.
-  apply @derives_trans with ((lseg x y * next y z) && (ewand (next z v) TT) *  next z v).
-  intros w [w1 [w2 [? [ ? ?]]]]. exists w1; exists w2; split3; auto. split; auto.
-  exists w2; exists w; split3; auto.
-  apply sepcon_derives; auto.
-  generalize (goedel_loeb (All x:adr,  
+  apply derives_trans with (((lseg x y * next y z) && (ewand (next z v) TT)) *  next z v).
+  apply exclude_elsewhere.
+  generalize (goedel_loeb (ALL x:adr,  
     lseg x y * next y z && ewand (next z v) TT >=> lseg x z) TT) ; intro.
   spec H.
-  2:  intros w ?; apply (H (@level _ R.ag_rmap w) I x w (le_refl _)); auto.
+Focus 2.
+  apply sepcon_derives; auto.
+  apply subp_e.
+  eapply derives_trans; [ apply H |].
+  apply allp_left with x. auto.
   clear.
   apply allp_right; intro x.
   apply subp_i1.
-  intros w [[_ ?] [? ?]].
-  rewrite lseg_unfold. left.
-  split.
-  do 3 red. intro; subst x.
-  clear - H0 H1.
-  destruct H1 as [w1 [w2 [? [? _]]]].
-  assert (app_pred (next z v * (lseg z y * next y z)) w2) by (do 2 eexists; split3; eauto).
-  rewrite <- sepcon_assoc in H2.
-  destruct H2 as [wa [wb [? [? ?]]]].
-  assert (app_pred (lseg z y * (next y z * next z v)) w2).
+  rewrite (lseg_unfold x z).
+  apply orp_right1.
+  apply andp_right.
+  apply not_prop_right; intro; subst x.
+  apply andp_left2.
+  apply derives_trans with ((EX u:_, (next z u * TT)) && ewand (next z v) TT).
+  apply andp_derives.
+  rewrite lseg_unfold.
+  rewrite distrib_orp_sepcon.
+  apply orp_left; normalize.
+  apply exp_right with tail. rewrite sepcon_assoc. apply sepcon_derives; normalize.
+  apply exp_right with z. apply sepcon_TT. auto.
+  normalize.
+  apply ewand_conflict.
   rewrite sepcon_comm.
+  rewrite <- sepcon_assoc.
+  apply derives_trans with (FF * TT); [ | normalize].
+  apply sepcon_derives; auto. 
+  apply next_conflict.
+
+   normalize.
+   match goal with |- ! ?P && _ |-- _ => remember P as S end.
+   rewrite (lseg_unfold x y).
+   rewrite andp_comm.
+  rewrite distrib_orp_sepcon.
+  rewrite distrib_orp_andp. 
+  rewrite distrib_orp_andp. 
+  apply orp_left. normalize. apply exp_right with tail.
+  apply derives_trans with (next x tail * (|>lseg tail y * next y z && ewand (next z v) TT && !S)).
+  rewrite andp_comm. rewrite <- andp_assoc.
   rewrite sepcon_assoc.
-  exists wb; exists wa; split3; auto.
-  clear - H5.
-  rewrite (lseg_unfold z y) in H5.
-  rewrite distrib_orp_sepcon in H5.
-  destruct H5.
-  repeat rewrite sepcon_andp_prop1 in H.
-  destruct H as [_ H].
-  repeat rewrite exp_sepcon1 in H.
-  destruct H as [u ?].
-  rewrite (sepcon_comm (next z u)) in H.
-  rewrite sepcon_assoc in H.
-  rewrite sepcon_comm in H.
-  rewrite (sepcon_comm (next y z)) in H.
-  rewrite <- sepcon_assoc in H.
-  rewrite sepcon_assoc in H.
-  destruct H as [w1 [w3 [? [? _]]]].
-  apply next_conflict in H0; auto.
-  rewrite sepcon_andp_prop1 in H. rewrite emp_sepcon in H.
-  destruct H. hnf in H. subst y.
-  apply next_conflict in H0; auto.
-  rewrite lseg_unfold in H0.
-  rewrite distrib_orp_sepcon in H0.
-  destruct H0.
-  repeat rewrite sepcon_andp_prop1 in H0.
-  destruct H0.
-  repeat rewrite exp_sepcon1 in H2.
-  destruct H2 as [u H2].
-  do 3 red in H0. exists u.
- rewrite later_allp in H.
-  specialize (H u).
-  rewrite sepcon_assoc in H2.
-  destruct H2 as [w1 [w2 [? [? ?]]]].
-  red in H. rewrite sub_later in H.
-  specialize (H w2).
-  spec H. apply join_level in H2; destruct H2; omega.
-  exists w1; exists w2; split3; auto.
-  apply H; auto.
-  rewrite later_andp. split.
-  rewrite later_sepcon.
-  eapply sepcon_derives; try apply H4; auto.
-  apply now_later.
-  eapply now_later; eauto.
-  clear - H2 H1.
-  destruct H1 as [w3 [w4 [? [? _]]]].
-  destruct (join_assoc H2 (join_com H)) as [f [? ?]].
-  exists w3; exists f; split3; auto.
-  exists z.
-  rewrite lseg_eq.
-  rewrite sepcon_andp_prop1 in H0.
-  destruct H0. hnf in H0; subst y.
-  rewrite sepcon_comm in H2.
-  eapply sepcon_derives; try apply H2; auto.
-  apply now_later.
+  rewrite unfash_sepcon_distrib.
+  eapply derives_trans; [eapply ewand_TT_sepcon | ].  
+  apply sepcon_derives; auto.
+  apply andp_left1. apply andp_left2; auto.
+  subst S.
+  apply andp_right. apply andp_right. apply andp_left1. apply andp_left2; auto.
+  apply andp_left2; auto.
+  apply andp_left1; auto. apply andp_left1;auto.
+  apply sepcon_derives; auto.
+  apply derives_trans with (|> (lseg tail y * next y z && ewand (next z v) TT) && !S).
+  apply andp_derives; auto.
+  repeat rewrite later_andp. rewrite later_sepcon.
+  apply andp_derives; auto. apply sepcon_derives; auto.
+   apply now_later. apply now_later.
+  subst.
+  rewrite <- later_unfash.
+  rewrite <- later_andp. apply later_derives.
+  apply derives_trans with (lseg tail y * next y z && ewand (next z v) TT &&
+           !( lseg tail y * next y z && ewand (next z v) TT >=> lseg tail z)).
+ apply andp_derives; auto. 
+ apply unfash_derives.
+ apply allp_left with tail. auto.
+ eapply derives_trans; [ eapply andp_derives; [ apply derives_refl | apply unfash_fash] | ].
+ apply modus_ponens.
+ normalize. apply exp_right with z.
+ apply andp_left1. apply andp_left1.
+ rewrite lseg_eq. apply derives_trans with (next x z * emp).
+  rewrite sepcon_emp; auto. apply sepcon_derives; auto.
+ apply now_later.
 Qed.
+
+ Lemma allp_andp1 {A}{NA: NatDed A}{B}: forall (any: B) (P: B -> A) Q,
+   allp P && Q = ALL x:B, P x && Q.
+Proof. intros. apply pred_ext. apply allp_right; intro x.
+   apply andp_derives; auto. apply allp_left with x; auto.
+   apply andp_right. apply allp_right; intro x; apply allp_left with x. 
+  apply andp_left1; auto. apply allp_left with any. apply andp_left2; auto.
+Qed.
+
 
 Lemma list_append:  (* U3 *)
    forall x y, lseg x y * lseg y 0 |-- lseg x 0.
 Proof.
  intros.
-  generalize (goedel_loeb (All x:adr, lseg x y * lseg y 0  >=> lseg x 0) TT) ; intro.
-  spec H; [ clear  | intros w ?; apply (H (@level _ R.ag_rmap w) I x w (le_refl _)); auto].
-  apply andp_left2.
-  apply allp_right; intro x.
+  generalize (loeb (ALL x:adr, lseg x y * lseg y 0  >=> lseg x 0)) ; intro.
+ apply subp_e.
+  eapply derives_trans; [ apply H; clear H | apply allp_left with x; auto].
+  apply allp_right; intro z.
   apply subp_i1.
-  intros w [? ?].
-  destruct (eq_dec x 0).
-  subst. rewrite lseg_eq.
-  rewrite lseg_unfold in H0.
-  rewrite distrib_orp_sepcon in H0.
-  destruct H0.
-  rewrite sepcon_andp_prop1 in H0. destruct H0.
-  rewrite exp_sepcon1 in H1.
-  destruct H1 as [u ?]. unfold next in H1.
-  repeat rewrite sepcon_andp_prop1 in H1.
-  destruct H1 as [H1 _]; hnf in H1. inv H1. 
-  rewrite sepcon_andp_prop1 in H0. destruct H0. hnf in H0. subst.
-  rewrite lseg_eq in H1. rewrite sepcon_emp in H1. auto.
-  rewrite (lseg_unfold x y) in H0.
-  rewrite distrib_orp_sepcon in H0.
-  destruct H0.
-  rewrite sepcon_andp_prop1 in H0. destruct H0.
-  rewrite exp_sepcon1 in H1.
-  destruct H1 as [z H1].
-  rewrite lseg_neq; auto.
-  exists z.
-  rewrite sepcon_assoc in H1.
-  rewrite later_allp in H.
-  specialize (H z).
-  destruct H1 as [w1 [w2 [? [? ?]]]].
-  red in H. rewrite sub_later in H.
-  specialize (H w2).
-  spec H. apply join_level in H1; destruct H1; omega.
-  exists w1; exists w2; split3; auto.
-  apply H; auto.
-  rewrite later_sepcon.
-  eapply sepcon_derives; try apply H3; auto.
-  apply now_later.
-  rewrite sepcon_andp_prop1 in H0.
-  destruct H0. hnf in H0; subst y. rewrite emp_sepcon in H1; auto.
+  match goal with |- ! |> ?S' && _ |-- _ => remember S' as S end.
+  rewrite (lseg_unfold z y).
+  rewrite distrib_orp_sepcon.
+  rewrite andp_comm.
+  rewrite distrib_orp_andp.
+  apply orp_left; normalize.
+  apply derives_trans with (next z tail * |> (lseg tail y * lseg y 0) && !|>S).
+  apply andp_derives; auto.
+  rewrite sepcon_assoc; apply sepcon_derives; auto.
+  rewrite later_sepcon; apply sepcon_derives; auto. apply now_later. 
+  rewrite (lseg_unfold z 0). apply orp_right1.
+  apply andp_right.
+  unfold next. normalize. apply prop_right. omega.
+  apply exp_right with tail.
+  rewrite andp_comm; rewrite unfash_sepcon_distrib.
+  apply sepcon_derives. apply andp_left2; auto.
+  rewrite <- later_unfash; rewrite <- later_andp; apply later_derives.
+  subst. rewrite unfash_allp.
+ rewrite allp_andp1; [ | apply 0].
+ apply allp_left with tail.
+ rewrite andp_comm.
+ eapply derives_trans; [ eapply andp_derives; [ apply derives_refl | apply unfash_fash] | ].
+ apply modus_ponens.
+  apply andp_left1; auto.
 Qed.
 
 Lemma lseg_U5:
@@ -446,7 +308,7 @@ Proof.
  intros.
  rewrite (lseg_neq z w); auto.
  repeat rewrite exp_sepcon2.
- apply exp_derives; intro v.
+ normalize. intro v. apply exp_right with v.
  repeat rewrite <- sepcon_assoc.
  apply sepcon_derives; auto.
  apply lseg_cons_in_next_context.
@@ -460,8 +322,7 @@ Proof.
   subst. rewrite lseg_eq. repeat  rewrite sepcon_emp. 
   eapply derives_trans; try apply list_append.
   apply sepcon_derives; eauto.
-  rewrite next_gt_0.
-  apply prop_andp_left; intro.
+  rewrite next_gt_0. normalize.
   apply next_lseg; omega.
   apply lseg_U5; auto.
 Qed.
