msl/examples/cont/seplog.v
@@ -1,26 +1,52 @@
 Require Import msl.examples.cont.language.
-Require Import msl.examples.cont.sep_base.
-Require Import msl.msl_standard.
-Require Import msl.rmaps.
-Require Import msl.rmaps_lemmas.
-Require Import msl.Coqlib2.
+Require Import msl.base.
+Require Import msl.seplog.
+Require Import msl.alg_seplog.
 
-Obligation Tactic := idtac.
-
-Local Open Scope pred.
-
-Hint Extern 3 (list_nodups _ = true) => (compute; reflexivity).
-Hint Extern 3 (typecheck _ _ = true) => (compute; reflexivity).
-Hint Extern 3 (expcheck _ _ = true) => (compute; reflexivity).
-Hint Resolve andb_true_intro.
+Local Open Scope logic.
 
 Module Type SEMAX.
+
+  Parameter mpred : Type.
+  Parameter Nm: NatDed mpred.  Existing Instance Nm.
+  Parameter Sm: SepLog mpred.  Existing Instance Sm.
+  Parameter Cm: ClassicalSep mpred.  Existing Instance Cm.
+  Parameter Im: Indir mpred.  Existing Instance Im.
+  Parameter Rm: RecIndir mpred.  Existing Instance Rm.
+  Parameter SIm: SepIndir mpred.  Existing Instance SIm.
+  Parameter SRm: SepRec mpred.  Existing Instance SRm.
+
+  Parameter mapsto: forall (v1 v2: adr), mpred.
+
+  Axiom mapsto_conflict:  forall a b c, mapsto a b  *  mapsto a c |-- FF.
+
+  Definition assert := env -> mpred.
+  Bind Scope logic with assert.
+
+  Definition funspec := (list var * assert)%type.
+  Definition funspecs := table adr funspec.
+
+  Definition call (P: list var * assert) (vl: list adr) : mpred := 
+     (!! (length vl = length (fst P)) && snd P (arguments (fst P) vl)). 
+  Parameter cont: forall (nP: funspec)  (v: adr), mpred.
+
+Definition funassert (G: funspecs) : mpred := 
+   (ALL  i:_, ALL P:_,  !! (table_get G i = Some P) --> cont P i)  && 
+   (ALL  i:_, ALL P:_,  cont P i --> !! exists P', table_get G i = Some P').
+
+
+  Axiom funassert_get:
+  forall G v nP,  funassert  G && cont nP v |--
+                      EX P':assert, (ALL vl:list adr, |> ! (call nP vl <=> call (fst nP,P') vl)) && !! (table_get G v = Some (fst nP,P')).
+
+  Parameter allocpool: forall (b: adr), mpred.
+  Axiom alloc: forall b, allocpool b = ((!! (b > 0) && mapsto b 0) * allocpool (S b)).
 
   Parameter semax : varset -> funspecs -> assert -> control -> Prop.
   Parameter semax_func: forall (G: funspecs) (p: program) (G': funspecs), Prop.
 
-Axiom semax_func_nil: forall G, semax_func G nil nil.
-Axiom semax_func_cons: 
+  Axiom semax_func_nil: forall G, semax_func G nil nil.
+  Axiom semax_func_cons: 
    forall  fs id f vars P (G G': funspecs),
       inlist id (map (@fst adr (list var * control)) fs) = false ->
       list_nodups vars = true ->
@@ -29,14 +55,14 @@ Axiom semax_func_cons:
       semax_func G fs G' ->
       semax_func G ((id, (vars,f))::fs) ((id, P) :: G').
 
-Definition program_proved (p: program) :=
+  Definition program_proved (p: program) :=
    exists G, semax_func G p G 
                             /\ table_get G 0 = Some  (0::nil, fun s => allocpool (eval (Var 0) s)).
 
-Axiom semax_sound: 
+  Axiom semax_sound: 
   forall p, program_proved p -> forall n, run p n <> None.
 
-Axiom semax_go:  forall vars G (P: funspec) x ys,   
+  Axiom semax_go:  forall vars G (P: funspec) x ys,   
     typecheck vars (Go x ys) = true ->
     semax vars G (fun s => cont P (eval x s) && call P (eval_list ys s)) (Go x ys) .
 
@@ -69,11 +95,11 @@ Axiom semax_pre:
 Axiom semax_exp: forall A vars G (P: A -> assert) c,
     typecheck vars c = true ->
     (forall v:A, semax vars G (P v) c) ->
-    semax vars G (fun s => Ex v:A, (P v s)) c.
+    semax vars G (fun s => EX v:A, (P v s)) c.
 
 Axiom semax_exp': forall A (any: A) vars G (P: A -> assert) c,
     (forall v:A, semax vars G (P v) c) ->
-    semax vars G (fun s => Ex v:A, (P v s)) c.
+    semax vars G (fun s => EX v:A, (P v s)) c.
 
 Axiom semax_prop:
   forall (R: Prop) vars G P c,
@@ -86,657 +112,6 @@ Axiom semax_G:
 
 
 End SEMAX.
-
-Module Semax : SEMAX.
-
-Local Open Scope pred.
-
-Definition guard (p: program) (G: funspecs) (vars: varset) (P : assert) (k: control) : pred nat :=
-     All s:env, P s && funassert G >=> assert_safe p vars k s.
-
-Record semaxArg :Type := SemaxArg {
- sa_vars: varset;
- sa_P: assert;
- sa_c: control
-}.
-
-Definition believe (semax: semaxArg -> pred nat) 
-      (p: program) (P: funspec) (f: adr) : pred nat :=
-      Ex k: list var * control, 
-        !!(table_get p f = Some k /\ length (fst k) = length (fst P) /\ list_norepet (fst k)) &&
-      |> semax (SemaxArg (fst k) (fun s => call P (map s (fst k))) (snd k)).
-
-Definition believe_all (semax: semaxArg -> pred nat) (G: funspecs) (p: program) (G': funspecs) : pred nat :=
-  All v:adr, All args: list var, All P: assert,
-     !! (table_get G' v = Some (args,P)) -->
-     believe semax p (args, fun s => P s && funassert G) v.
-
-Definition semax_ (semax: semaxArg -> pred nat) (a: semaxArg) : pred nat :=
- match a with SemaxArg vars P c =>
-     All p: program, All G: funspecs, believe_all semax G p G --> guard p G vars P c
-  end.
-
-Lemma prop_imp {A}{agA: ageable A}: 
-  forall (P: Prop) (Q: pred A) w, (P -> app_pred Q w) -> app_pred (!!P --> Q) w.
-Proof. repeat intro. specialize (H H1). eapply pred_nec_hereditary; eauto.
-Qed.
-
-
-Lemma HOcontractive_semax_ : HOcontractive semax_.
-Proof.
-  auto 50 with contractive.
-Qed.
-
-Definition semax'  := HORec semax_.
-
-Lemma semax'_unfold: forall vars P c,
-     semax' (SemaxArg vars P c) = 
-         All p: program, All G:funspecs, believe_all semax' G p G --> guard p G vars P c.
-Proof.
-  intros. 
-  unfold semax' at 1. rewrite HORec_fold_unfold; auto.
-  apply HOcontractive_semax_.
-Qed.
-
-Definition semax vars (G: funspecs) (P: assert) (k: control) : Prop := 
-       typecheck vars k = true /\ forall n,  semax' (SemaxArg vars (fun s => P s && funassert G) k) n.
-
-Definition semax_func (G: funspecs) (p: program) (G': funspecs) :=
-    match_specs p G' /\ 
-    forall n, believe_all semax' G p G' n.
-
-Lemma semax_func_nil: forall G, semax_func G nil nil.
-Proof. split; repeat intro. constructor. inv H0. Qed.
-
-Lemma semax_func_cons: 
-   forall  fs id f vars P (G G': funspecs),
-      inlist id (map (@fst adr (list var * control)) fs) = false ->
-      list_nodups vars = true ->
-      length vars = length (fst P) ->
-      semax vars G (fun s => call P (map s vars)) f ->
-      semax_func G fs G' ->
-      semax_func G ((id, (vars,f))::fs) ((id, P) :: G').
-Proof.
-intros until G'. intros H0 H Hlen ? ?.
-apply inlist_notIn in H0.
-destruct H2.
-split.
-constructor; auto.
-destruct H1; auto.
-intro.
-specialize (H3 n).
-intros b nargs' Q.
-specialize (H3 b nargs' Q).
-intros ? ? ?.
-destruct (eq_dec id b).
-subst.
-Focus 2.
-specialize (H3 _ H4).
-spec H3.
-clear - H5 n0.
-hnf in H5|-*.
-unfold table_get  in H5; fold @table_get in H5.
-rewrite if_false in H5; auto.
-clear H5.
-destruct H3 as [k [? ?]]; exists k; split; auto.
-unfold table_get; fold @table_get.
-rewrite if_false; auto.
-(* End Focus 2 *)
-unfold table_get in H5; fold @table_get in H5.
-rewrite if_true in H5; auto.
-simpl in H5.
-inv H5.
-exists (vars,f).
-split.
-simpl.
-rewrite if_true; auto. split; auto. split; auto. apply nodups_norepet. auto.
-simpl fst; simpl snd.
-hnf; intros.
-destruct H1 as [_ H1].
-specialize (H1 a'0).
-replace (fun s : env =>
-           call (nargs', fun s0 : env => Q s0 && funassert G) (map s vars))
- with (fun s : env => call (nargs', Q) (map s vars) && funassert G).
-apply H1.
-extensionality s. forget (map s vars) as vl.
-clear.
-apply pred_ext; intros ? ?.
-destruct H as [[? ?] ?].
-split. apply H. simpl snd in *. split; auto.
-destruct H. simpl fst in *; simpl snd in *.
-destruct H0; split; auto. split; auto.
-Qed.
-
-Lemma semax_G:
-   forall vars G P c, semax vars G (fun s => P s && funassert G) c -> semax vars G P c.
-Proof. 
-  intros. destruct H; split; auto.
-  intro; specialize (H0 n).
-  replace (fun s : env => P s && funassert G) with (fun s : env => P s && funassert G && funassert G);
-       auto.
-  extensionality s.
-  rewrite andp_assoc. f_equal. apply andp_dup.
-Qed.
-
-Lemma semax_go:  forall vars G (P: funspec) x ys,   
-    typecheck vars (Go x ys) = true ->
-    semax vars G (fun s => cont P (eval x s) && call P (eval_list ys s)) (Go x ys) .
-Proof.
- intros. rename H into TC.
-  split; auto.
-   intro n; hnf.
-   rewrite semax'_unfold.
-  intros p G0.
-  hnf. intros n' ? ?.
-  clear n H.
-  intros s w ? w' ?.
-  rewrite andp_assoc.
-  intros [[H4 H5] [_ GUARDIAN]].
-  pose (H3:=True).
-  clear G. rename G0 into G.
-  remember (eval x s) as v'.
-  destruct (funassert_get G v' P w') as [P' [H2 H2']].
-  split; auto.
-  generalize (H0 _ _ _ _ (necR_refl _) H2'); intro. clear H2'.
-  destruct H6 as [[formals k] [[H6 [H6' H6'']] ?]]. 
-  hnf in H6.
- rewrite semax'_unfold in H7.
-  apply assert_safe0; intros w'' Hw''.
-  assert (LATER: laterR n' (level w'')).
-    apply later_nat; apply necR_level in H1; apply age_level in Hw''.
-   unfold R.rmap in *; omega. specialize (H2 (eval_list ys s)).
-  red in H2. red in H2. red in H2.
-  specialize (H2 _ (t_step _ _ _ _ Hw'' )).
-  specialize (H7 _ LATER).
-  apply (pred_nec_hereditary _ _ _ (laterR_necR LATER)) in H0.
-  specialize (H7 p G _ (necR_refl _) H0). clear H0.
-  simpl fst in *. simpl snd in *.
-  do 3 red in H2.
-  apply (pred_hereditary _ _ _ Hw'') in H5.
-  specialize (H2 _ (le_refl _)).
-  specialize (H7 (locals2env (mk_locals formals (eval_list ys s))) _ (le_refl _) _ (necR_refl _)).
-  clear n' H LATER.
-  intros ? ? VC L H. rewrite <- L in *. clear L s. rename s' into s.
-  assert (step p (s,h, Go x ys) = Some ((mk_locals formals (eval_list ys (locals2env s)), h), k)).
-  simpl.
-  simpl typecheck in TC.
-  rewrite andb_true_iff in TC; destruct TC as [TC1 TC2].
-  rewrite (eval_expr_get vars s h x); auto. rewrite <- Heqv'.
-  simpl. rewrite H6.  simpl. 
-  rewrite (eval_expr_get_list vars s h ys); auto.
-  rename Hw'' into H12.
-  rewrite (age_level _ _ H12).
-  rewrite (safeN_step _ _ _ _ H0).
-  clear w H1.
-  pose (H11:=True).
-  spec H7.
-  eapply pred_hereditary in GUARDIAN; eauto.
-  split; auto.
-  split.
-  hnf. rewrite map_length. simpl fst. auto.
-  split; auto.
-  destruct H2 as [? _]. 
-  specialize (H1 _ (necR_refl _) H5).
-  simpl.
-  unfold call in H1. simpl in H1.
-  Transparent arguments.
-  unfold arguments in *.
-  Opaque arguments.
-  replace (map (locals2env (mk_locals formals (eval_list ys (locals2env s)))) formals)
-     with (eval_list ys (locals2env s)); [ apply H1 | ].
-  destruct H5 as [Hlen H5]. hnf in Hlen.
-  assert (length (eval_list ys (locals2env s)) = length formals).
-    rewrite H6'. auto.
-  forget (eval_list ys (locals2env s)) as vs.
-  clear - H2 H6''.
-  revert vs H2; induction H6''; intros; destruct vs; inv H2; simpl; auto.
-  f_equal. unfold locals2env; simpl. rewrite if_true by auto. auto.
- pattern vs at 1; rewrite (IHH6'' vs) by auto.
- forget (mk_locals tl vs) as y.
- clear - H. induction tl; simpl; auto. f_equal; simpl.
- unfold locals2env; simpl.
- rewrite if_false by (contradict H; simpl in *; intuition). auto.
- apply IHtl. intuition.
-  apply H7; auto.
-  apply varcompat_mk_locals. unfold eval_list. rewrite map_length. rewrite H6'; auto.
-  destruct H5 as [H5 _]; hnf in H5.
-  rewrite <- H5.
-  clear. induction ys; simpl; omega.
-  eapply pred_hereditary; eauto.
-Qed.
-
-Lemma semax_assign: forall x y c vars G P,
-    expcheck vars y = true ->
-    semax (vs_add x vars) G P c -> 
-    semax vars G (fun s => |> subst x (eval y s) P s) (Do x := y ; c).
-Proof.
- intros until P; intros TC [TC' ?].
- split.
- simpl in *. destruct y; inv TC; simpl; auto; try rewrite TC'; try rewrite H1; auto.
- intro; intros.
- unfold subst.
- rewrite semax'_unfold.
- intros p G' n' ? ? s w ? w' ? [[H6 H6'] H4].
- pose (H5:=True).
- apply assert_safe0; intros w'' ?.
- intros s' h VC L ?. rewrite <- L in *; clear L s; rename s' into s.
- generalize (age_level _ _ H7); intro. rewrite H9.
- apply (pred_hereditary _ _ _ H7) in H8.
- specialize (H6 _ (t_step _ _ _ _ H7)).
- apply (pred_hereditary _ _ _ H7) in H4.
- assert (necR n' (level w')). apply necR_trans with (level w); auto.
- apply nec_nat. auto. apply necR_level'. auto.
- apply (pred_nec_hereditary _ _ _ H10) in H1.
- clear n' w H3 H2 H0 H10.
- hnf in H5.
- assert (step p ((s,h), Do (Var x) := y; c) = Some ((table_set x (eval y (locals2env s)) s, h), c)).
- simpl. rewrite (eval_expr_get vars s h y); auto.
- apply (safeN_step _ _ _ _ H0).
-  specialize (H (@level _ ag_rmap w')). rewrite semax'_unfold in H.
- specialize (H p G' _ (necR_refl _) H1).
- specialize (H (locals2env (@table_set var _ EqDec_var x (eval y (locals2env s)) s))).
- specialize (H w''). spec H; [rewrite H9; omega | ].
- specialize (H _ (necR_refl _)).
- spec H. split; auto. 
- replace  (locals2env (table_set x (eval y (locals2env s)) s))
-   with (env_set (locals2env s) x (eval y (locals2env s))); auto.
-  split; [ auto | eapply pred_hereditary; eauto]. 
-  clear.
-   extensionality i. unfold env_set. unfold locals2env at 3.
-   destruct (eq_dec i x). subst. rewrite table_gss; auto. rewrite table_gso; auto.
- apply H; auto.
-  clear - VC.
-  intros i ?. destruct (eq_dec i x). subst. rewrite table_gss. congruence.
-  rewrite table_gso by auto. apply (VC i).
-  unfold vs_mem in H. apply ListSet.set_mem_correct1 in H.
-  apply ListSet.set_mem_correct2. unfold vs_add in H.
-  apply ListSet.set_add_elim2 in H; auto.
-Qed.
-
-Lemma semax_if: forall x c1 c2 vars G (P: assert),
-    expcheck vars x = true ->
-    semax vars G (fun s => !!(eval x s <> 0) && P s) c1 ->
-    semax vars G (fun s => !! (eval x s = 0) && P s) c2 ->
-    semax vars G (fun s => P s) (If x Then c1 Else c2).
-Proof.
- intros. rename H into TC.
- destruct H0 as [TC0 H]; destruct H1 as [TC1 H'].
- split.
- simpl; auto.
- intro.
- rewrite semax'_unfold.
- intros p G' n' ? ? s w ? w' ? [H5 H4].
- pose (H6:=True).
- apply assert_safe0; intros w'' ?.
- intros s' h VC L ?. rewrite <- L in *; clear L s; rename s' into s.
- generalize (age_level _ _ H7); intro. rewrite H9.
- destruct (eq_dec (eval x (locals2env s)) 0).
- (* zero *)
- clear H; rename H' into H.
- subst.
- assert (step p ((s,h), If x Then c1 Else c2) = Some ((s,h), c2)).
- simpl. rewrite (eval_expr_get vars s h x); auto. rewrite e; simpl; auto.
- apply (safeN_step _ _ _ _ H10).
- specialize (H n'). rewrite semax'_unfold in H.
- assert (necR n' (level w')). apply necR_trans with (level w); auto.
- apply nec_nat. auto. apply necR_level'. auto.
- specialize (H p G' _ H11 (pred_nec_hereditary _ _ _ H11 H1)).
- specialize (H (locals2env s) w'').
- spec H. omega.
- specialize (H _ (necR_refl _)).
- spec H.
-  rewrite andp_com.
- split. eapply pred_hereditary; eauto.
- apply (pred_hereditary _ _ _ H7) in H5.
- rewrite andp_assoc; split; [ |  apply H5].
- hnf; auto.
- apply H; auto.
- apply (pred_nec_hereditary _ _ _ (rt_step _ _ _ _ H7)); auto. 
- (* nonzero *)
- subst.
- assert (step p ((s,h), If x Then c1 Else c2) = Some ((s,h), c1)).
- simpl. rewrite (eval_expr_get vars s h x); auto. simpl.  rewrite if_false; auto.
- apply (safeN_step _ _ _ _ H10).
- specialize (H n'). rewrite semax'_unfold in H.
- assert (necR n' (level w')). apply necR_trans with (level w); auto.
- apply nec_nat. auto. apply necR_level'. auto.
- specialize (H p G' _ H11 (pred_nec_hereditary _ _ _ H11 H1)).
- specialize (H (locals2env s) w'').
- spec H. omega.
- specialize (H _ (necR_refl _)).
- spec H.
- rewrite andp_com.
- split. eapply pred_hereditary; eauto.
- apply (pred_hereditary _ _ _ H7) in H5.
- rewrite andp_assoc; split; [ |  apply H5].
- hnf; auto.
- apply H; auto.
- apply (pred_nec_hereditary _ _ _ (rt_step _ _ _ _ H7)); auto. 
-Qed.
-
-Lemma semax_load: forall x y z c vars G P,
-    expcheck vars y = true ->
-    semax (vs_add x vars) G P c -> 
-    semax vars G (fun s => ((mapsto (eval y s) z) * TT) && |> subst x z P s)
-               (Do x := Mem y ; c).
-Proof.
- intros until P. intros TC [TC' ?].
- split.
- simpl; auto.
- intro n.
- rewrite semax'_unfold.
- intros p G' n' ? ? s w ? w' ? [H5 H4].
- destruct H5 as [[? HP] HG].
- unfold subst in HP.
- apply assert_safe0; intros w'' H7.
- specialize (HP _ (t_step _ _ _ _ H7)).
- intros s' h VC L ?. rewrite <- L in *; clear s L; rename s' into s.
- generalize (age_level _ _ H7); intro. rewrite H8.
- assert (step p ((s,h), Do x := Mem y; c) = Some ((table_set x z s, h), c)).
- simpl. rewrite (eval_expr_get vars s h y); auto. simpl.
- replace (heap_get h (eval y (locals2env s))) with (Some z).
- auto.
- symmetry.
- apply H6. apply mapsto_e1; auto.
- apply (safeN_step _ _ _ _ H9). clear H9.
- specialize (H n'). rewrite semax'_unfold in H.
- assert (necR n' (level w')). apply necR_trans with (level w); auto.
- apply nec_nat. auto. apply necR_level'. auto.
- specialize (H p G' _ H9 (pred_nec_hereditary _ _ _ H9 H1)).
- specialize (H (locals2env (@table_set _ _ EqDec_var x z s)) w'').
- spec H.    unfold R.rmap in *; omega. 
- specialize (H _ (necR_refl _)).
- spec H. split; [split|].
-  rewrite locals2env_table_set. eauto.
-  eapply pred_hereditary; eauto.
-  eapply pred_hereditary; eauto.
- apply H; auto.
- apply varcompat_add; auto.
- eapply pred_hereditary; eauto.
-Qed.
-
-Lemma semax_store: forall x y v c vars G (P: assert),
-    expcheck vars x = true ->
-    expcheck vars y = true ->
-    semax vars G (fun s => mapsto (eval x s) (eval y s) * P s) c ->
-    semax vars G (fun s => mapsto (eval x s) v  * P s)  (Do Mem x  := y ; c).
-Proof.
- intros until P; intros TCx TCy [TC ?].
- split.
- simpl; auto.
- intro. rewrite semax'_unfold.
- intros p G' n' ? ? s w ? w' ? [[H5 H6] H4].
- apply assert_safe0; intros w'' ?.
- intros s' h VC L ?. rewrite <- L in *; clear L s; rename s' into s.
- generalize (age_level _ _ H7); intro. rewrite H9.
- assert (step p ((s,h), Do Mem x := y; c) = Some ((s, heap_set (eval x (locals2env s)) (eval y (locals2env s)) h), c)).
- simpl. rewrite (eval_expr_get vars s h y); auto. rewrite (eval_expr_get vars s h x); auto.
- apply (safeN_step _ _ _ _ H10).
- specialize (H n'). rewrite semax'_unfold in H.
- assert (necR n' (level w')). apply necR_trans with (level w); auto.
- apply nec_nat. auto. apply necR_level'. auto.
- specialize (H p G' _ H11 (pred_nec_hereditary _ _ _ H11 H1)).
- apply (pred_hereditary _ (level w') (level w'')) in H;
-   [ |  apply age_level in H7; rewrite H7; hnf; simpl; auto].
- apply (pred_hereditary _ _ _ H7) in H5.
- apply (pred_hereditary _ _ _ H7) in H6.
- apply (pred_hereditary _ _ _ H7) in H4.
- apply (pred_hereditary _ _ _ H7) in H8.
- clear H1; pose (H1:=True). clear n H0. pose (H0:=True).
- clear n' H2 H11. pose (H2:=True). pose (H11:=True).
- simpl in H8.
-clear w' H7 H9 H3. 
- pose (H7:=True); pose (H9:=True); pose (H3:=True).
- clear H0 H1.
- destruct H5 as [wa [wb [H0 [HP H1]]]].
- pose (m' := singleton_rmap (eval x (locals2env s)) (eval y (locals2env s)) w'').
- assert (joins m' wb).
- apply resource_at_joins2. unfold m'.
- rewrite singleton_rmap_level.
- apply join_level in H0. destruct H0. auto.
- unfold m'. intro i.
- clear - HP H0.
- apply (resource_at_join _ _ _ i) in H0.
- specialize (HP i).
- unfold singleton_rmap. rewrite resource_at_make_rmap.
- destruct (eq_dec i (eval x (locals2env s))). subst; rewrite if_true in HP; auto.
- exists (YES pfullshare (VAL (eval y (locals2env s))) NoneP).
- rewrite HP in *. inv H0; try pfullshare_join. constructor.
- rewrite if_false in HP by auto. 
- exists (wb @ i). 
- apply HP in H0. rewrite H0.
- rewrite <- core_resource_at. apply core_unit.
- destruct H5 as [ww H12].
- replace (level w'') with (level ww) in H.
- Focus 2.
- transitivity (level wb).
- apply join_level in H12. destruct H12 as [H12 H13]. symmetry ; apply H13.
- apply join_level in H0; destruct H0; auto.
- specialize (H (locals2env s) ww).
- spec H. simpl. apply le_refl.
- specialize (H _ (necR_refl _)).
- spec H. rewrite andp_assoc. rewrite andp_com.
- clear - H4 H0 HP H12 H6 H1.
- assert (app_pred ((mapsto (eval x (locals2env s)) v * TT) && (funassert G && funassert G')) w'').
- split; auto. exists wa; exists wb; split3; auto. split; auto.
- destruct H as [? _].
- split.
- apply join_com in H0. apply join_com in H12. apply join_core in H0. apply join_core in H12.
- apply funassert_core in H6. apply funassert_core in H4. rewrite H12 in H0.
- split; apply funassert_core; rewrite H0; auto.
- destruct H as [wa' [wb' [? [? ?]]]].
- assert (wa' = wa). eapply mapsto_uniq; eauto.
- apply join_core in H0; apply join_core in H. rewrite H0; rewrite H. auto. 
- subst wa'. generalize (join_canc (join_com H0) (join_com H)); intro; subst wb'.
-  generalize (singleton_rmap_mapsto (eval x (locals2env s)) (eval y (locals2env s)) w''); intro.
- assert (app_pred (mapsto (eval x (locals2env s)) (eval y (locals2env s)) * (TT && (funassert G && funassert G'))) ww).
- exists m'; exists wb; split3; auto.
- split; auto.
- apply join_com in H0. apply join_com in H12. apply join_core in H0. apply join_core in H12.
-  apply funassert_core in H6. apply funassert_core in H4.
- split; apply funassert_core; rewrite H0; auto.
- exists m'; exists wb; split3; auto.
- replace (level w'') with (level ww).
- Focus 2. simpl. transitivity (level wb).
- clear - H12; apply join_level in H12; destruct H12; symmetry; apply H0.
- clear - H0; apply join_level in H0; destruct H0; apply H0.
- apply H; auto.
- intros i v0. specialize (HP i).
- simpl.
- apply (resource_at_join _ _ _ i) in H12.
- unfold m' in *; clear m'.
- unfold singleton_rmap in H12.
- rewrite resource_at_make_rmap in H12.
- change AV.address with adr in H12.
-  specialize (H8 i v0). simpl in H8. 
-
-  destruct (eq_dec i (eval x (locals2env s))). 
-  subst. rewrite heap_gss.
-  apply join_unit2_e in H12. rewrite <- H12.
-  split; intro Hx; inv Hx; auto.
-  apply YES_join_full in H12; auto.
-  rewrite H12. apply NO_identity.
-  apply join_unit1_e in H12; [ | rewrite <- core_resource_at; apply core_identity].
-  rewrite heap_gso; auto. 
- apply (resource_at_join _ _ _ i) in H0.
- rewrite <- H12.
- apply HP in H0. rewrite H0; auto.
-Qed.
-
-Lemma semax_pre: 
-  forall P P' vars G c, (forall s, P s |-- P' s) -> semax vars G P' c -> semax vars G P c.
-Proof.
- intros. destruct H0 as [TC H0]; split; auto.
- intro n; specialize (H0 n).
- rewrite semax'_unfold in *.
- intros p G'. specialize (H0 p G').
- intros n' ? ?. specialize (H0 _ H1 H2).
- intros s w ? ? ? ?. specialize (H0 s _ H3 _ H4).
- apply H0.
- destruct H5; split; auto. destruct H5;  split; auto. apply H; auto.
-Qed.
-
-
-Lemma semax_exp: forall {A} vars G (P: A -> assert) c,
-    typecheck vars c = true ->
-    (forall v:A, semax vars G (P v) c) ->
-    semax vars G (fun s => Ex v:A, (P v s)) c.
-Proof.
- intros ? ? ? ? ? TC ?.
- split; auto. 
- intro.
- rewrite semax'_unfold.
- intros p G'. intros n' ? ?.
- intros s. intros ? ?. intros ? ?. intros [[[v ?] ?] ?].
- specialize (H v). destruct H as [_ H].
- rewrite semax'_unfold in H. eapply H; eauto. split; auto. split; auto.
-Qed.
-
-Lemma semax_exp': forall {A} (any: A) vars G (P: A -> assert) c,
-    (forall v:A, semax vars G (P v) c) ->
-    semax vars G (fun s => Ex v:A, (P v s)) c.
-Proof.
- intros ? ? ? ? ? ?.
- split; auto. 
- destruct (H any); auto.
- intro.
- rewrite semax'_unfold.
- intros p G'. intros n' ? ?.
- intros s. intros ? ?. intros ? ?. intros [[[v ?] ?] ?].
- specialize (H v). destruct H as [_ H].
- rewrite semax'_unfold in H. eapply H; eauto. split; auto. split; auto.
-Qed.
-
-Lemma semax_prop:
-  forall (R: Prop) vars G P c,
-      typecheck vars c = true ->
-      (R -> semax vars G P c) ->
-      semax vars G (fun s => !! R && P s) c.
-Proof.
-  intros R vars G P c TC ?. split; auto. intro n.  rewrite semax'_unfold. intros p G'.
-  intros n' ? ? b w ? w' ? [[[? ?] ?] ?].
-  destruct (H H4).
-  specialize (H9 n). rewrite semax'_unfold in H9.
-  eapply H9; eauto. split; auto. split; auto.
-Qed.
-
-Definition program_proved (p: program) :=
-   exists G, semax_func G p G  /\ table_get G 0 = Some (0::nil, fun s => allocpool (eval (Var 0) s)).
-
-Lemma semax_sound: 
-  forall p, program_proved p -> forall n, run p n <> None.
-Proof.
-  intros.
-  destruct H as [G [[? ?] ?]].
-  generalize (funassert_make_world p G n); intro.
-  destruct (semax_go nil G  (0::nil, fun s => allocpool (eval (Var 0) s))
-                (Const 0) (Const (boundary p) :: nil) (eq_refl _)) as [_ ?].
-  specialize (H3 n).
-  rewrite semax'_unfold in H3.
-  specialize (H3 p G _ (necR_refl _) (H0 _) (locals2env nil) 
-                    (make_world G (initial_heap p) n)).
-  spec H3. rewrite level_make_world. auto.
-  specialize (H3 _ (necR_refl _)).
-  spec H3.
-  split; auto.
-  split; auto.
-  split.
-  apply (funassert_e _ _ _ H1 _ H2).
-  unfold call.
-  Transparent arguments. unfold arguments. Opaque arguments.
-  simpl snd.
-  unfold locals2env, table_get. rewrite if_true; auto.
-  split. simpl; auto.
-  apply allocpool_make_world; auto.
-  hnf in H3.
-  specialize (H3 nil (initial_heap p)).
-  spec H3. intros i ?. inv H4.
-  spec H3. auto.
-  spec H3. apply cohere_make_world; auto.
-  unfold run; intro.
-  destruct H3 as [sk' ?].
-  rewrite level_make_world in H3. 
- unfold locals,table, var,adr in H3,H4. rewrite H3 in H4; inv H4.
-Qed.
-
-End Semax.
-
-Import Semax.
-
-(* PROOF AUTOMATION FOR SEMAX *)
-
-Hint Extern 3 (inlist _ _ = false) => (compute; reflexivity).
-
-Lemma arguments_gss: forall x xl v vl, arguments (x::xl)(v::vl) x = v.
-Proof.
-  intros.  
- Transparent arguments. unfold arguments, locals2env,mk_locals;  simpl.
- Opaque arguments.
-  rewrite if_true; auto.
-Qed.
-Lemma arguments_gso: forall x xl v vl x', x<>x' -> arguments (x::xl)(v::vl)x' = arguments xl vl x'.
-Proof.
-  intros.  
- Transparent arguments. unfold arguments, locals2env,mk_locals;  simpl.
- Opaque arguments.
-  rewrite if_false; auto.
-Qed.
-
-Ltac compute_neq := solve [let H := fresh in intro H; inversion H].
-
-Hint Rewrite arguments_gss : args.
-Hint Rewrite arguments_gso using compute_neq : args.
-
-Ltac call_tac := unfold call; simpl; autorewrite with args; simpl.
-
-Ltac funassert_tac := 
-  match goal with 
-  | |-   ?A && ?B |-- _ =>
-      match A with context [funassert _] => apply andp_left1; funassert_tac  end ||
-      match B with context [funassert _] => apply andp_left2; funassert_tac  end
-  | |- funassert _ |-- _ => apply funassert_e; simpl; reflexivity
- end.
-
-Ltac func_tac := 
-   apply semax_func_cons; 
-    [ compute; reflexivity | compute; reflexivity | compute; reflexivity 
-    |  (*eapply semax_pre; [intro ; call_tac; apply derives_refl | ] *)
-    | ].                     
-
-Ltac rewrite' H := eapply semax_pre; [ intro; rewrite H; apply derives_refl | ].
-
-(* This tactic works but introduces magic wands, which is undesirable *)
-Ltac forward_magic := 
-  match goal with |- semax _ ?G ?P (Assign (Mem ?e1) ?e2 ?c) =>
-      let v := fresh "v" in
-        (evar (v:adr);
-       apply semax_pre with (P' := fun s => mapsto (eval e1 s) v * (mapsto (eval e1 s) v -* P s));
-               [intro | apply semax_store; auto  ] );
-       unfold v; clear v
-  end.
-
-Ltac forward := 
- match goal with
- | |- semax _ _ _ (language.If _ _ _) =>
-          apply semax_if; [ compute; reflexivity | | ]
- | |- semax _ _ _ (Assign (Mem _) _ _) => 
-            eapply semax_store; [ compute ; reflexivity | compute; reflexivity | reflexivity | ]
- | |- semax _ _ ?P (Go ?x ?ys) =>
-  apply semax_G;
-  let p := fresh "P" in 
-   evar (p: funspec);
-   eapply semax_pre with (fun s => cont p (eval x s) && call p (eval_list ys s));
-       [ intro; apply andp_right 
-       | apply semax_go; [ compute; reflexivity ] ]; unfold p; clear p;
-       [ try funassert_tac | call_tac  ]; simpl
- end.
-
-Hint Resolve now_later sepcon_derives.
-
-
-
-Definition semax_body (G: funspecs) (spec: funspec) (f: list var * control) :=
-  semax (fst f) G (fun s => call spec (map s (fst f))) (snd f).
 
 
 
