msl/examples/cont/client_lemmas.v
@@ -1,0 +1,133 @@
+Require Import msl.examples.cont.language.
+Require Import msl.base.
+Require Import msl.seplog.
+Require Import msl.alg_seplog.
+Require Import msl.examples.cont.seplog.
+Require Import msl.examples.cont.lseg.
+Require Import msl.Coqlib2.
+Require Import msl.log_normalize.
+
+Local Open Scope logic.
+
+
+Import Semax.
+
+(* PROOF AUTOMATION FOR SEMAX *)
+
+Hint Extern 3 (inlist _ _ = false) => (compute; reflexivity).
+
+Lemma arguments_gss: forall x xl v vl, arguments (x::xl)(v::vl) x = v.
+Proof.
+  intros.  
+ Transparent arguments. unfold arguments, locals2env,mk_locals;  simpl.
+ Opaque arguments.
+  rewrite if_true; auto.
+Qed.
+Lemma arguments_gso: forall x xl v vl x', x<>x' -> arguments (x::xl)(v::vl)x' = arguments xl vl x'.
+Proof.
+  intros.  
+ Transparent arguments. unfold arguments, locals2env,mk_locals;  simpl.
+ Opaque arguments.
+  rewrite if_false; auto.
+Qed.
+
+Ltac compute_neq := solve [let H := fresh in intro H; inversion H].
+
+Hint Rewrite arguments_gss : args.
+Hint Rewrite arguments_gso using compute_neq : args.
+
+Ltac call_tac := unfold call; simpl; autorewrite with args; simpl.
+
+
+Lemma funassert_e:  forall G i f,
+      table_get G i = Some f -> 
+      funassert G |-- cont f i.
+Proof.
+  intros.
+  unfold funassert.
+  apply andp_left1.
+  apply allp_left with i. apply allp_left with f.
+  normalize.
+  eapply derives_trans with (TT && (TT --> cont f i)).
+  apply andp_right; auto. apply TT_right. apply modus_ponens.
+Qed.
+
+Ltac funassert_tac := 
+  match goal with 
+  | |-   ?A && ?B |-- _ =>
+      match A with context [funassert _] => apply andp_left1; funassert_tac  end ||
+      match B with context [funassert _] => apply andp_left2; funassert_tac  end
+  | |- funassert _ |-- _ => apply funassert_e; simpl; reflexivity
+ end.
+
+Ltac func_tac := 
+   apply semax_func_cons; 
+    [ compute; reflexivity | compute; reflexivity | compute; reflexivity 
+    |  (*eapply semax_pre; [intro ; call_tac; apply derives_refl | ] *)
+    | ].                     
+
+Ltac rewrite' H := eapply semax_pre; [ intro; rewrite H; apply derives_refl | ].
+
+(* This tactic works but introduces magic wands, which is undesirable *)
+Ltac forward_magic := 
+  match goal with |- semax _ ?G ?P (Assign (Mem ?e1) ?e2 ?c) =>
+      let v := fresh "v" in
+        (evar (v:adr);
+       apply semax_pre with (P' := fun s => mapsto (eval e1 s) v * (mapsto (eval e1 s) v -* P s));
+               [intro | apply semax_store; auto  ] );
+       unfold v; clear v
+  end.
+
+Ltac forward := 
+ match goal with
+ | |- semax _ _ _ (IfThenElse _ _ _) =>
+          apply semax_if; [ compute; reflexivity | | ]
+ | |- semax _ _ _ (Assign (Mem _) _ _) => 
+            eapply semax_store; [ compute ; reflexivity | compute; reflexivity | reflexivity | ]
+ | |- semax _ _ ?P (Go ?x ?ys) =>
+  apply semax_G;
+  let p := fresh "P" in 
+   evar (p: funspec);
+   eapply semax_pre with (fun s => cont p (eval x s) && call p (eval_list ys s));
+       [ intro; apply andp_right 
+       | apply semax_go; [ compute; reflexivity ] ]; unfold p; clear p;
+       [ try funassert_tac | call_tac  ]; simpl
+ end.
+
+Hint Resolve now_later sepcon_derives.
+
+
+
+Definition semax_body (G: funspecs) (spec: funspec) (f: list var * control) :=
+  semax (fst f) G (fun s => call spec (map s (fst f))) (snd f).
+
+
+Lemma semax_store_next: forall x y v c vars G (Q P: assert),
+    expcheck vars x = true ->
+    expcheck vars y = true ->
+    Q = (fun s => next (eval x s) v  * P s) ->
+    semax vars G (fun s => next (eval x s) (eval y s) * P s) c ->
+    semax vars G Q  (Do Mem x  := y ; c).
+Proof. intros; subst. 
+    apply semax_pre with (fun s => mapsto (eval x s) v * (!! (eval x s > 0) && P s)).
+    intros. unfold next. rewrite sepcon_andp_prop. 
+    rewrite sepcon_comm. rewrite sepcon_andp_prop. rewrite sepcon_comm; auto.
+    apply semax_store; auto.
+    eapply semax_pre; try apply H2.
+    intros; unfold next.
+    rewrite sepcon_andp_prop. 
+    rewrite (sepcon_comm (andp _ _)). rewrite sepcon_andp_prop.
+   rewrite sepcon_comm; auto.
+ Qed.
+
+Lemma semax_load_next: forall x y z c vars G P,
+    expcheck vars y = true ->
+    semax (vs_add x vars) G P c -> 
+    semax vars G (fun s => (next (eval y s) z * TT) && |> subst x z P s)
+               (Do x := Mem y ; c).
+Proof.
+ intros.
+  apply semax_pre with (fun s => mapsto (eval y s) z * TT && |> subst x z P s).
+ intros. apply andp_derives; auto. apply sepcon_derives; auto. apply andp_left2; auto.
+ apply semax_load; auto.
+Qed.
