msl/examples/cont/model.v
@@ -1,0 +1,1073 @@
+Require Import msl.msl_standard.
+Require Import msl.Coqlib2.
+Require Import msl.rmaps.
+Require Import msl.rmaps_lemmas.
+Require Import msl.examples.cont.language.
+Require Import msl.examples.cont.seplog.
+
+Hint Extern 3 (list_nodups _ = true) => (compute; reflexivity).
+Hint Extern 3 (typecheck _ _ = true) => (compute; reflexivity).
+Hint Extern 3 (expcheck _ _ = true) => (compute; reflexivity).
+Hint Resolve andb_true_intro.
+
+Obligation Tactic := idtac.
+
+Module Semax : SEMAX.
+
+Local Open Scope pred.
+
+(******  CONSTRUCTION OF rmap FOR THE CONT LANGUAGE *****)
+Inductive kind := VAL: adr -> kind | FUN: list var -> kind.
+
+Module AV0 <: ADR_VAL0.
+ Definition address := adr.
+ Definition some_address := 0.
+ Definition kind := kind.
+End AV0.
+
+Module AV := SimpleAdrVal AV0.
+Module R := Rmaps AV.
+Module RML := Rmaps_Lemmas R.
+Export RML. Export R.
+Instance Cross_rmap : Cross_alg rmap := Cross_rmap_simple (fun _ => I).
+
+Obligation Tactic := idtac.
+
+(******  MAPSTO AND RELATED OPERATORS *****)
+
+Program Definition mapsto (v1 v2: adr) : pred rmap :=
+  fun w => forall i,
+         if eq_dec i v1 then w @ i = YES pfullshare (VAL v2) NoneP else identity (w @ i).
+Next Obligation.
+ intros. intros ? ? ? ?.
+  intro i; specialize (H0 i).
+  destruct (eq_dec i v1).
+  apply (age1_YES _ _ _ _ _ H); auto.
+  destruct (identity_resource (a @ i)) as [? _]. specialize (H1 H0).
+  apply identity_resource. 
+  generalize (age1_resource_at _ _ H i (a @ i)); intro.
+  generalize (resource_at_approx a i); intro. 
+  destruct (a @ i); try contradiction.
+  rewrite H2; simpl in *; auto.
+  rewrite H2; simpl in *; auto.
+Qed.
+
+Lemma mapsto_conflict:
+   forall a b c, mapsto a b  *  mapsto a c |-- FF.
+  Proof.
+    intros.
+    intros w  [w1 [w2 [? [? ?]]]]; hnf.
+    specialize (H0 a). specialize (H1 a).
+    rewrite if_true in * by auto.
+    apply (resource_at_join _ _ _ a) in H.
+    rewrite H0 in H; rewrite H1 in H; inv H.
+    pfullshare_join.
+ Qed.
+
+Lemma singleton_rmap_OK: 
+   forall v v' m,  
+       resource_fmap (approx (level m))
+            oo (fun i => if eq_dec i v then YES pfullshare (VAL v') NoneP else core m @  i) =
+    (fun i => if eq_dec i v then YES pfullshare (VAL v') NoneP else core m @ i).
+Proof.
+  intros; extensionality i; unfold compose; simpl.
+  destruct (eq_dec i v). 
+  unfold resource_fmap. f_equal. apply preds_fmap_NoneP.
+  rewrite <- level_core.
+  symmetry; apply resource_at_approx.
+Qed.
+
+Definition singleton_rmap  (v v': adr) (m: rmap) : rmap :=
+  proj1_sig 
+  (make_rmap (fun i => if eq_dec i v then YES pfullshare (VAL v') NoneP  else core m @ i ) 
+    I (level m) (singleton_rmap_OK _ _ m)).
+
+Lemma singleton_rmap_level: forall x y m,
+      level (singleton_rmap x y m) = level m.
+Proof. 
+  intros.  apply level_make_rmap.
+Qed.
+
+Lemma singleton_rmap_mapsto:
+   forall x y n, app_pred (mapsto x y) (singleton_rmap x y n).
+ Proof.
+  intros. hnf. simpl snd.
+  unfold singleton_rmap.
+  intro; repeat rewrite resource_at_make_rmap.
+  change AV.address with adr.
+ destruct (eq_dec i x); auto.
+ apply resource_at_core_identity.
+Qed.
+
+Local Open Scope pred.
+
+Lemma mapsto_uniq: forall (x y: adr) w w', core w = core w' -> mapsto x y w -> mapsto x y w' -> w=w'.
+Proof.
+  intros.
+ apply rmap_ext.
+ assert (level (core w) = level (core w')) by congruence.
+ do 2 rewrite level_core in H2. auto.
+ intro. 
+ specialize (H0 l); specialize (H1 l).
+ destruct (@eq_dec adr _ l x); try congruence.
+ apply identity_unit_equiv in H0.
+ apply unit_core in H0.
+ apply identity_unit_equiv in H1.
+ apply unit_core in H1.
+ rewrite core_resource_at in *. congruence.
+Qed.
+
+Lemma mapsto_e1: forall v1 v2 w,
+       app_pred (mapsto v1 v2 * TT) w ->
+       w @ v1 = YES pfullshare (VAL v2) NoneP.
+Proof.
+ intros.
+ destruct H as [w1 [w2 [? [? ?]]]].
+ hnf in H0.
+ specialize (H0 v1).
+ apply (resource_at_join _ _ _ v1) in H.
+ rewrite if_true in H0 by auto. rewrite H0 in H.
+apply join_YES_pfullshare1 in H. inv H; auto.
+Qed.
+
+Definition assert := env -> pred rmap.
+Bind Scope pred with assert.
+
+(****** PROGRAM SAFETY AS A SEPARATION-LOGIC PREDICATE *)
+
+Program Definition cohere (concrete: heap) : pred rmap :=
+ fun w =>
+ forall p v, heap_get (concrete) p = Some v  <->
+                 w @ p = YES pfullshare (VAL v) NoneP.
+Next Obligation.
+  unfold hereditary; intros.
+  rewrite H0. 
+  apply age1_YES; auto.
+Qed.
+
+
+Program Definition assert_safe 
+     (p: program) (vars: varset) (ctl: control) : assert :=
+  fun s w => forall s' h, varcompat vars s' -> 
+                   locals2env s' = s -> cohere h w -> safeN p (s',h,ctl) (level w).
+ Next Obligation.
+  unfold hereditary; intros.
+  eapply safeN_less; [ | apply H0]; auto. subst.
+  apply age_level in H.   rewrite H. change R.rmap with rmap. omega.
+  clear - H H3. hnf in H3|-*. intros. rewrite H3.
+    generalize (age1_YES _ _ p pfullshare (VAL v) H); intros.
+  intuition.
+ Qed.
+
+Lemma assert_safe0: 
+        forall p vars k s w, 
+           (forall w', age w w' -> app_pred (assert_safe p vars k s) w) ->
+            app_pred (assert_safe p vars k s) w.
+Proof.
+  intros.
+  case_eq (age1 w); intros.
+  apply (H _ H0).
+  hnf; repeat intro.
+  rewrite age1_level0 in H0. rewrite H0. hnf. econstructor; reflexivity.
+Qed.
+
+(******* FUNASSERT, MAKE_WORLD ********************)
+
+Definition funspec := (list var * assert)%type.
+Definition funspecs := table adr funspec.
+
+Definition unpack (P: list adr -> pred rmap) (vl: listprod (@cons Type (list adr) nil)):  pred rmap := P (fst vl).
+
+Definition call (P: list var * assert) (vl: list adr) : pred rmap := 
+     (!! (length vl = length (fst P)) && snd P (arguments (fst P) vl)).
+
+Program Definition cont (nP: funspec)  (v: adr) : pred rmap :=
+  fun w => w @ v = PURE (FUN (fst nP)) (preds_fmap (approx (level w)) (SomeP (list adr::nil) 
+             (unpack (call nP)))).
+Next Obligation.
+ intros; intro; intros.
+  apply (age1_resource_at a a' H v (PURE (FUN (fst nP)) _));   simpl; auto.
+Qed.
+
+Definition funassert (G: funspecs) : pred rmap := 
+   (ALL  i:_, ALL P:_,  !! (table_get G i = Some P) --> cont P i)  && 
+   (ALL  i:_, ALL P:_,  cont P i --> !! exists P', table_get G i = Some P').
+
+Definition make_world_aux (G: funspecs) (h: heap) (n: nat) (a: adr) : resource :=
+   match table_get G a with
+   | Some P => PURE (FUN (fst P))
+                               (preds_fmap (approx n) 
+                                      (SomeP (@cons Type (list adr) nil) (unpack (call P))))
+   | None => match heap_get h a with
+                     | Some v => YES pfullshare (VAL v) NoneP
+                     | None => NO
+                    end
+   end.
+
+Lemma make_world_aux_OK:
+  forall G h n, 
+         resource_fmap (approx n) oo make_world_aux G h n =  make_world_aux G h n.
+Proof.
+ intros.
+ extensionality v; 
+ unfold make_world_aux, compose.
+ destruct (table_get G v). destruct f as [nargs P]. simpl.
+ f_equal. f_equal. rewrite <- compose_assoc. rewrite approx_oo_approx. auto.
+ destruct (heap_get h v); auto.
+ unfold resource_fmap.
+ f_equal. apply preds_fmap_NoneP.
+Qed.  
+
+Definition make_world (G: funspecs) (h: heap) (n: nat) : rmap :=
+    proj1_sig (make_rmap (make_world_aux G h n) I n (make_world_aux_OK _ _ _)).
+
+Lemma level_make_world:
+  forall h G n, level (make_world G h n) = n.
+Proof.
+ intros; simpl.
+ apply level_make_rmap.
+Qed.
+
+Inductive match_specs: forall (p: program) (G: funspecs), Prop :=
+| match_specs_nil: match_specs nil nil
+| match_specs_cons: forall i vars f p' P G',
+         not (In i (map (@fst _ _) p')) ->
+         match_specs p' G' ->
+         typecheck vars f = true ->
+         match_specs ((i,(vars,f))::p') ((i,P)::G').
+
+Lemma match_specs_boundary:
+   forall p G i, 
+   match_specs p G -> i >= boundary p -> table_get G i = None.
+Proof.
+  induction 1. intros. reflexivity.
+  intros. simpl in *. 
+  destruct (@eq_dec adr _ i i0). subst.
+  clear - H2. destruct (boundary p'). elimtype False; omega.
+ generalize (Max.le_max_l i0 n); intro. elimtype False. omega.
+ apply IHmatch_specs.
+ destruct (boundary p'); try omega.
+ generalize (Max.le_max_r i0 n0);  omega.
+Qed.
+
+Lemma funassert_e:  forall G i f,
+      table_get G i = Some f -> 
+      funassert G |-- cont f i.
+Proof.
+  intros.
+  unfold funassert.
+  apply andp_left1.
+  intros w ?. apply H0; auto.
+Qed.
+
+Lemma funassert_make_world: forall p G n,
+         app_pred (funassert G) (make_world G (initial_heap p) n).
+Proof.
+ intros ? ? ?.
+ forget (initial_heap p) as h.
+ split.
+ intros i P w ? ?.
+ hnf in H0.
+ eapply pred_nec_hereditary; try apply H.
+ clear w H.
+ hnf. unfold make_world; simpl. rewrite resource_at_make_rmap.
+ unfold make_world_aux. rewrite H0.
+ f_equal. simpl. f_equal. rewrite level_make_rmap.
+ reflexivity.
+ intros i P w ? ?.
+ hnf.
+ case_eq (table_get G i); intros. eauto.
+ elimtype False.
+ hnf in H0.
+ case_eq (make_world G h n @ i); intros.
+ apply (necR_NO _ _ i H) in H2. inversion2 H0 H2.
+ apply (necR_YES _ _ i _ _ _ H) in H2. inversion2 H2 H0.
+ clear dependent w.
+ unfold make_world in H2.
+ rewrite resource_at_make_rmap in H2. unfold make_world_aux in H2.
+ rewrite H1 in H2. destruct (heap_get h i); inv H2.
+Qed.
+
+Lemma cohere_make_world: 
+  forall p G n,  
+      match_specs p G ->
+     app_pred (cohere (initial_heap p)) (make_world G (initial_heap p) n).
+Proof.
+ intros.
+ hnf.
+ intros. unfold make_world, make_world_aux; simpl. rewrite resource_at_make_rmap.
+ unfold  initial_heap. simpl. unfold heap_get.
+  rename p0 into i.
+ destruct (lt_dec i (boundary p)).
+ split; intro. inv H0. elimtype False.
+ revert H0; case_eq (table_get G i); intros. destruct f as [nargs P].
+ inv H1. inv H1.
+ rewrite (match_specs_boundary p G i); auto; try omega.
+ split; intro Hx; inv Hx; auto.
+Qed.
+
+Lemma funassert_get:
+  forall G v nP,  funassert  G && cont nP v |--
+                      EX P':assert, (ALL vl:list adr, |> ! (call nP vl <=> call (fst nP,P') vl)) && !! (table_get G v = Some (fst nP,P')).
+Proof.
+ intros. intros w [? ?].
+ destruct H.
+ specialize (H v); specialize (H1 v).
+ specialize (H1 _ _ (necR_refl _) H0).
+ destruct H1 as [[args P'] ?].
+ exists P'.
+ specialize (H _ _ (necR_refl _) H1).
+ split.
+ Focus 2. hnf in H,H0. inversion2 H H0. apply H1.
+ clear H1. rename H into H99. rename H0 into H97.
+ hnf in H99,H97. rewrite H99 in H97.  apply PURE_inj in H97. destruct H97 as [H H97].
+ simpl in H. destruct nP as [na P]. inv H.
+ intro vl. intros w' ? w'' ?.
+  assert (level w'' < level w). do 3 red in H. apply laterR_level in H. 
+       apply le_lt_trans with (level w'); auto.
+ simpl fst.
+  split; intros w''' ? ?.  
+ match type of H97 with ?A = _ => assert (app_pred (A (vl,tt)) w''') end.
+  rewrite H97.
+ split.
+  change rmap with R.rmap in *.
+  change ag_rmap with R.ag_rmap in *. 
+  apply necR_level in H2; omega.
+ apply H3.
+  destruct H4. apply H5.
+ match type of H97 with _ = ?A => assert (app_pred (A (vl,tt)) w''') end.
+  rewrite <- H97.
+ split.
+  change rmap with R.rmap in *.
+  change ag_rmap with R.ag_rmap in *. 
+  apply necR_level in H2; omega.
+ apply H3.
+  destruct H4. apply H5.
+Qed.
+
+Lemma cont_core: forall P i w, app_pred (cont P i) w <-> app_pred (cont P i) (core w).
+Proof.
+ intros.
+ unfold cont. simpl. rewrite <- core_resource_at.
+ split; intro. rewrite H.
+ clear. symmetry. rewrite level_core. apply unit_core; constructor.
+ rewrite level_core in H.
+ generalize (core_unit (w @ i)); intro.
+ rewrite H in H0.
+ inv H0; auto.
+Qed.
+
+Lemma funassert_core: forall G w, app_pred (funassert G) w <-> app_pred (funassert G) (core w).
+Proof.
+ intros.
+ split; intros [? ?]; split; intros i P w' ? ?.
+ specialize (H i P _ (necR_refl _) H2).
+ apply cont_core in H. eapply pred_nec_hereditary; eauto.
+ generalize (core_unit w); intro.
+ unfold unit_for in H3.
+ eapply nec_join in H3; eauto.
+ destruct H3 as [y' [z' [? [? ?]]]].
+ generalize (necR_linear' H4 H5); intro.
+ spec H6. apply join_level in H3. destruct H3; congruence.
+ subst z'. clear H5.
+ specialize (H0 i P _ H4).
+ apply join_core in H3. rewrite cont_core in H2. rewrite H3 in H2. rewrite <- cont_core in H2.
+ specialize (H0 H2). apply H0.
+ assert (necR (core w) (core w')).
+ generalize (core_unit w); intro.
+ unfold unit_for in H3.
+ apply join_comm in H3.
+ eapply nec_join in H3; eauto.
+ destruct H3 as [y' [z' [? [? ?]]]].
+ generalize (necR_linear' H1 H5); intro.
+ spec H6. apply join_level in H3. destruct H3; congruence. subst z'.
+ apply join_comm in H3.
+ generalize (unit_identity _ H3); intro.
+ apply identity_unit_equiv in H6. apply unit_core in H6.
+ apply join_core in H3. rewrite H6 in H4. rewrite H3 in H4; auto.
+ specialize (H i P _ H3 H2).
+ apply cont_core in H; auto.
+ assert (necR (core w) (core w')).
+ generalize (core_unit w); intro.
+ unfold unit_for in H3.
+ apply join_comm in H3.
+ eapply nec_join in H3; eauto.
+ destruct H3 as [y' [z' [? [? ?]]]].
+ generalize (necR_linear' H1 H5); intro.
+ spec H6. apply join_level in H3. destruct H3; congruence. subst z'.
+ apply join_comm in H3.
+ generalize (unit_identity _ H3); intro.
+ apply identity_unit_equiv in H6. apply unit_core in H6.
+ apply join_core in H3. rewrite H6 in H4. rewrite H3 in H4; auto.
+ specialize (H0 i P _ H3).
+ apply H0. rewrite <- cont_core; auto.
+Qed.
+
+
+(**************** ALLOCPOOL ***************************)
+
+
+Program Definition allocpool (b: adr) : pred rmap :=
+   fun w => b>0 /\ forall i, if lt_dec i b then identity (w @ i) else w @ i = YES pfullshare (VAL 0) NoneP.
+Next Obligation.
+ intros. intro; intros.
+  destruct H0; split; auto.
+ intro i; specialize (H1 i).
+ destruct (lt_dec i b).
+  eapply age1_resource_at_identity; eauto.
+ apply (age1_YES _ _ _ _ _ H); auto.
+Qed.
+
+Lemma allocpool_make_world: forall p G n,
+          match_specs p G ->
+          app_pred (allocpool (boundary p)) (make_world G (initial_heap p) n).
+Proof.
+  unfold make_world; intros.
+  rename H into H'.
+ unfold initial_locals,initial_heap  in *.
+ split.
+ destruct p; simpl. omega. destruct p. destruct (boundary p0); omega. 
+ intro loc.
+ destruct (make_rmap
+        (make_world_aux G
+           (fun i : adr => if lt_dec i (boundary p) then None else Some 0) n)
+        I n
+        (make_world_aux_OK G
+           (fun i : adr => if lt_dec i (boundary p) then None else Some 0) n)) as [? [? ?]];
+  simpl in *. rewrite e0. unfold make_world_aux.
+ unfold heap_get.
+ destruct (lt_dec loc (boundary p)).
+ destruct (table_get G loc);  apply identity_resource; auto.
+ rewrite (match_specs_boundary p G loc); auto.
+ omega.
+Qed.
+
+Lemma alloc: forall b, allocpool b = ((!! (b > 0) && mapsto b 0) * allocpool (S b)).
+Proof.
+ intros. apply pred_ext.
+  intros w ?.
+ destruct H as [H' H]. 
+  destruct (deallocate w 
+                   (fun i => if lt_dec b i then NO else w @ i) 
+                   (fun i => if eq_dec b i then NO else w @ i)
+               I I) as [w1 [w2 [? ?]]].
+ intro l; specialize (H l).
+ destruct (eq_dec b l). subst. rewrite if_false by omega. rewrite if_false in H by omega.
+ rewrite H; constructor.
+ destruct (lt_dec b l).
+ rewrite if_false in H by omega.
+ rewrite H; constructor.
+ rewrite if_true in H.
+ apply identity_unit_equiv in H. apply H.
+ unfold adr in *; omega.
+ exists w1; exists w2; split3; auto.
+ split; auto.
+ intro i. apply (resource_at_join _ _ _ i) in H0. specialize (H i). rewrite H1 in *.
+ clear w1 H1.
+ destruct (lt_dec b i).
+ rewrite if_false by omega. apply NO_identity.
+ destruct (eq_dec i b). subst. rewrite if_false in H by omega. auto.
+ rewrite if_true in H. auto.
+ unfold adr in *; omega.
+ split. omega.
+ intro i. apply (resource_at_join _ _ _ i) in H0. specialize (H i). rewrite H1 in *.
+ clear w1 H1.
+ destruct (lt_dec b i).
+ rewrite if_false by omega. rewrite if_false in H by omega. rewrite H in H0. inv H0; auto.
+ rewrite if_true by omega.
+ destruct (eq_dec i b). subst. rewrite if_false in H by omega. rewrite H in H0; inv H0; auto.
+ apply NO_identity. pfullshare_join.
+ rewrite if_true in H by (unfold adr in *; omega).
+ apply H in H0. rewrite H0; auto.
+
+  intros w [w1 [w2 [? [? ?]]]].
+  destruct H0 as [H0' H0]. destruct H1 as [_ H1].
+ split; auto.
+  intro i. specialize (H0 i); specialize (H1 i). apply (resource_at_join _ _ _ i) in H.
+  destruct (lt_dec i b). rewrite if_true in H1 by omega.
+  rewrite if_false in H0 by omega. apply H0 in H. rewrite <- H; auto.
+  destruct (@eq_dec adr _ i b). subst. rewrite H0 in H. rewrite if_true in H1 by omega.
+  apply join_comm in H. apply H1 in H. auto.
+  rewrite if_false in H1. rewrite H1 in H. apply H0 in H. auto.
+  unfold AV.address, AV0.address, adr in *. omega.
+Qed.
+
+Require msl.seplog msl.alg_seplog.
+Definition mpred : Type := predicates_hered.pred rmap.
+Instance Nm: seplog.NatDed mpred := alg_seplog.algNatDed rmap.
+Instance Sm: seplog.SepLog mpred := alg_seplog.algSepLog rmap.
+Instance Cm: seplog.ClassicalSep mpred := alg_seplog.algClassicalSep rmap.
+Instance Im: alg_seplog.Indir mpred := alg_seplog.algIndir rmap.
+Instance Rm: alg_seplog.RecIndir mpred := alg_seplog.algRecIndir rmap.
+Instance SIm: alg_seplog.SepIndir mpred := alg_seplog.algSepIndir rmap.
+Instance SRm: alg_seplog.SepRec mpred := alg_seplog.algSepRec rmap.
+
+Definition guard (p: program) (G: funspecs) (vars: varset) (P : assert) (k: control) : pred nat :=
+     ALL s:env, P s && funassert G >=> assert_safe p vars k s.
+
+Record semaxArg :Type := SemaxArg {
+ sa_vars: varset;
+ sa_P: assert;
+ sa_c: control
+}.
+
+Definition believe (semax: semaxArg -> pred nat) 
+      (p: program) (P: funspec) (f: adr) : pred nat :=
+      EX k: list var * control, 
+        !!(table_get p f = Some k /\ length (fst k) = length (fst P) /\ list_norepet (fst k)) &&
+      |> semax (SemaxArg (fst k) (fun s => call P (map s (fst k))) (snd k)).
+
+Definition believe_all (semax: semaxArg -> pred nat) (G: funspecs) (p: program) (G': funspecs) : pred nat :=
+  ALL v:adr, ALL args: list var, ALL P: assert,
+     !! (table_get G' v = Some (args,P)) -->
+     believe semax p (args, fun s => P s && funassert G) v.
+
+Definition semax_ (semax: semaxArg -> pred nat) (a: semaxArg) : pred nat :=
+ match a with SemaxArg vars P c =>
+     ALL p: program, ALL G: funspecs, believe_all semax G p G --> guard p G vars P c
+  end.
+
+Lemma prop_imp {A}{agA: ageable A}: 
+  forall (P: Prop) (Q: pred A) w, (P -> app_pred Q w) -> app_pred (!!P --> Q) w.
+Proof. repeat intro. specialize (H H1). eapply pred_nec_hereditary; eauto.
+Qed.
+
+
+Lemma HOcontractive_semax_ : HOcontractive semax_.
+Proof.
+  auto 50 with contractive.
+Qed.
+
+Definition semax'  := HORec semax_.
+
+Lemma semax'_unfold: forall vars P c,
+     semax' (SemaxArg vars P c) = 
+         ALL p: program, ALL G:funspecs, believe_all semax' G p G --> guard p G vars P c.
+Proof.
+  intros. 
+  unfold semax' at 1. rewrite HORec_fold_unfold; auto.
+  apply HOcontractive_semax_.
+Qed.
+
+Definition semax vars (G: funspecs) (P: assert) (k: control) : Prop := 
+       typecheck vars k = true /\ forall n,  semax' (SemaxArg vars (fun s => P s && funassert G) k) n.
+
+Definition semax_func (G: funspecs) (p: program) (G': funspecs) :=
+    match_specs p G' /\ 
+    forall n, believe_all semax' G p G' n.
+
+Lemma semax_func_nil: forall G, semax_func G nil nil.
+Proof. split; repeat intro. constructor. inv H0. Qed.
+
+Lemma semax_func_cons: 
+   forall  fs id f vars P (G G': funspecs),
+      inlist id (map (@fst adr (list var * control)) fs) = false ->
+      list_nodups vars = true ->
+      length vars = length (fst P) ->
+      semax vars G (fun s => call P (map s vars)) f ->
+      semax_func G fs G' ->
+      semax_func G ((id, (vars,f))::fs) ((id, P) :: G').
+Proof.
+intros until G'. intros H0 H Hlen ? ?.
+apply inlist_notIn in H0.
+destruct H2.
+split.
+constructor; auto.
+destruct H1; auto.
+intro.
+specialize (H3 n).
+intros b nargs' Q.
+specialize (H3 b nargs' Q).
+intros ? ? ?.
+destruct (eq_dec id b).
+subst.
+Focus 2.
+specialize (H3 _ H4).
+spec H3.
+clear - H5 n0.
+hnf in H5|-*.
+unfold table_get  in H5; fold @table_get in H5.
+rewrite if_false in H5; auto.
+clear H5.
+destruct H3 as [k [? ?]]; exists k; split; auto.
+unfold table_get; fold @table_get.
+rewrite if_false; auto.
+(* End Focus 2 *)
+unfold table_get in H5; fold @table_get in H5.
+rewrite if_true in H5; auto.
+simpl in H5.
+inv H5.
+exists (vars,f).
+split.
+simpl.
+rewrite if_true; auto. split; auto. split; auto. apply nodups_norepet. auto.
+simpl fst; simpl snd.
+hnf; intros.
+destruct H1 as [_ H1].
+specialize (H1 a'0).
+replace (fun s : env =>
+           call (nargs', fun s0 : env => Q s0 && funassert G) (map s vars))
+ with (fun s : env => call (nargs', Q) (map s vars) && funassert G).
+apply H1.
+extensionality s. forget (map s vars) as vl.
+clear.
+apply pred_ext; intros ? ?.
+destruct H as [[? ?] ?].
+split. apply H. simpl snd in *. split; auto.
+destruct H. simpl fst in *; simpl snd in *.
+destruct H0; split; auto. split; auto.
+Qed.
+
+Lemma semax_G:
+   forall vars G P c, semax vars G (fun s => P s && funassert G) c -> semax vars G P c.
+Proof. 
+  intros. destruct H; split; auto.
+  intro; specialize (H0 n).
+  replace (fun s : env => P s && funassert G) with (fun s : env => P s && funassert G && funassert G);
+       auto.
+  extensionality s.
+  rewrite andp_assoc. f_equal. apply andp_dup.
+Qed.
+
+Lemma semax_go:  forall vars G (P: funspec) x ys,   
+    typecheck vars (Go x ys) = true ->
+    semax vars G (fun s => cont P (eval x s) && call P (eval_list ys s)) (Go x ys) .
+Proof.
+ intros. rename H into TC.
+  split; auto.
+   intro n; hnf.
+   rewrite semax'_unfold.
+  intros p G0.
+  hnf. intros n' ? ?.
+  clear n H.
+  intros s w ? w' ?.
+  rewrite andp_assoc.
+  intros [[H4 H5] [_ GUARDIAN]].
+  pose (H3:=True).
+  clear G. rename G0 into G.
+  remember (eval x s) as v'.
+  destruct (funassert_get G v' P w') as [P' [H2 H2']].
+  split; auto.
+  generalize (H0 _ _ _ _ (necR_refl _) H2'); intro. clear H2'.
+  destruct H6 as [[formals k] [[H6 [H6' H6'']] ?]]. 
+  hnf in H6.
+ rewrite semax'_unfold in H7.
+  apply assert_safe0; intros w'' Hw''.
+  assert (LATER: laterR n' (level w'')).
+    apply later_nat; apply necR_level in H1; apply age_level in Hw''.
+   unfold R.rmap in *; omega. specialize (H2 (eval_list ys s)).
+  red in H2. red in H2. red in H2.
+  specialize (H2 _ (t_step _ _ _ _ Hw'' )).
+  specialize (H7 _ LATER).
+  apply (pred_nec_hereditary _ _ _ (laterR_necR LATER)) in H0.
+  specialize (H7 p G _ (necR_refl _) H0). clear H0.
+  simpl fst in *. simpl snd in *.
+  do 3 red in H2.
+  apply (pred_hereditary _ _ _ Hw'') in H5.
+  specialize (H2 _ (le_refl _)).
+  specialize (H7 (locals2env (mk_locals formals (eval_list ys s))) _ (le_refl _) _ (necR_refl _)).
+  clear n' H LATER.
+  intros ? ? VC L H. rewrite <- L in *. clear L s. rename s' into s.
+  assert (step p (s,h, Go x ys) = Some ((mk_locals formals (eval_list ys (locals2env s)), h), k)).
+  simpl.
+  simpl typecheck in TC.
+  rewrite andb_true_iff in TC; destruct TC as [TC1 TC2].
+  rewrite (eval_expr_get vars s h x); auto. rewrite <- Heqv'.
+  simpl. rewrite H6.  simpl. 
+  rewrite (eval_expr_get_list vars s h ys); auto.
+  rename Hw'' into H12.
+  rewrite (age_level _ _ H12).
+  rewrite (safeN_step _ _ _ _ H0).
+  clear w H1.
+  pose (H11:=True).
+  spec H7.
+  eapply pred_hereditary in GUARDIAN; eauto.
+  split; auto.
+  split.
+  hnf. rewrite map_length. simpl fst. auto.
+  split; auto.
+  destruct H2 as [? _]. 
+  specialize (H1 _ (necR_refl _) H5).
+  simpl.
+  unfold call in H1. simpl in H1.
+  Transparent arguments.
+  unfold arguments in *.
+  Opaque arguments.
+  replace (map (locals2env (mk_locals formals (eval_list ys (locals2env s)))) formals)
+     with (eval_list ys (locals2env s)); [ apply H1 | ].
+  destruct H5 as [Hlen H5]. hnf in Hlen.
+  assert (length (eval_list ys (locals2env s)) = length formals).
+    rewrite H6'. auto.
+  forget (eval_list ys (locals2env s)) as vs.
+  clear - H2 H6''.
+  revert vs H2; induction H6''; intros; destruct vs; inv H2; simpl; auto.
+  f_equal. unfold locals2env; simpl. rewrite if_true by auto. auto.
+ pattern vs at 1; rewrite (IHH6'' vs) by auto.
+ forget (mk_locals tl vs) as y.
+ clear - H. induction tl; simpl; auto. f_equal; simpl.
+ unfold locals2env; simpl.
+ rewrite if_false by (contradict H; simpl in *; intuition). auto.
+ apply IHtl. intuition.
+  apply H7; auto.
+  apply varcompat_mk_locals. unfold eval_list. rewrite map_length. rewrite H6'; auto.
+  destruct H5 as [H5 _]; hnf in H5.
+  rewrite <- H5.
+  clear. induction ys; simpl; omega.
+  eapply pred_hereditary; eauto.
+Qed.
+
+Lemma semax_assign: forall x y c vars G P,
+    expcheck vars y = true ->
+    semax (vs_add x vars) G P c -> 
+    semax vars G (fun s => |> subst x (eval y s) P s) (Do x := y ; c).
+Proof.
+ intros until P; intros TC [TC' ?].
+ split.
+ simpl in *. destruct y; inv TC; simpl; auto; try rewrite TC'; try rewrite H1; auto.
+ intro; intros.
+ unfold subst.
+ rewrite semax'_unfold.
+ intros p G' n' ? ? s w ? w' ? [[H6 H6'] H4].
+ pose (H5:=True).
+ apply assert_safe0; intros w'' ?.
+ intros s' h VC L ?. rewrite <- L in *; clear L s; rename s' into s.
+ generalize (age_level _ _ H7); intro. rewrite H9.
+ apply (pred_hereditary _ _ _ H7) in H8.
+ specialize (H6 _ (t_step _ _ _ _ H7)).
+ apply (pred_hereditary _ _ _ H7) in H4.
+ assert (necR n' (level w')). apply necR_trans with (level w); auto.
+ apply nec_nat. auto. apply necR_level'. auto.
+ apply (pred_nec_hereditary _ _ _ H10) in H1.
+ clear n' w H3 H2 H0 H10.
+ hnf in H5.
+ assert (step p ((s,h), Do (Var x) := y; c) = Some ((table_set x (eval y (locals2env s)) s, h), c)).
+ simpl. rewrite (eval_expr_get vars s h y); auto.
+ apply (safeN_step _ _ _ _ H0).
+  specialize (H (@level _ ag_rmap w')). rewrite semax'_unfold in H.
+ specialize (H p G' _ (necR_refl _) H1).
+ specialize (H (locals2env (@table_set var _ EqDec_var x (eval y (locals2env s)) s))).
+ specialize (H w''). spec H; [rewrite H9; omega | ].
+ specialize (H _ (necR_refl _)).
+ spec H. split; auto. 
+ replace  (locals2env (table_set x (eval y (locals2env s)) s))
+   with (env_set (locals2env s) x (eval y (locals2env s))); auto.
+  split; [ auto | eapply pred_hereditary; eauto]. 
+  clear.
+   extensionality i. unfold env_set. unfold locals2env at 3.
+   destruct (eq_dec i x). subst. rewrite table_gss; auto. rewrite table_gso; auto.
+ apply H; auto.
+  clear - VC.
+  intros i ?. destruct (eq_dec i x). subst. rewrite table_gss. congruence.
+  rewrite table_gso by auto. apply (VC i).
+  unfold vs_mem in H. apply ListSet.set_mem_correct1 in H.
+  apply ListSet.set_mem_correct2. unfold vs_add in H.
+  apply ListSet.set_add_elim2 in H; auto.
+Qed.
+
+Lemma semax_if: forall x c1 c2 vars G (P: assert),
+    expcheck vars x = true ->
+    semax vars G (fun s => !!(eval x s <> 0) && P s) c1 ->
+    semax vars G (fun s => !! (eval x s = 0) && P s) c2 ->
+    semax vars G (fun s => P s) (If x Then c1 Else c2).
+Proof.
+ intros. rename H into TC.
+ destruct H0 as [TC0 H]; destruct H1 as [TC1 H'].
+ split.
+ simpl; auto.
+ intro.
+ rewrite semax'_unfold.
+ intros p G' n' ? ? s w ? w' ? [H5 H4].
+ pose (H6:=True).
+ apply assert_safe0; intros w'' ?.
+ intros s' h VC L ?. rewrite <- L in *; clear L s; rename s' into s.
+ generalize (age_level _ _ H7); intro. rewrite H9.
+ destruct (eq_dec (eval x (locals2env s)) 0).
+ (* zero *)
+ clear H; rename H' into H.
+ subst.
+ assert (step p ((s,h), If x Then c1 Else c2) = Some ((s,h), c2)).
+ simpl. rewrite (eval_expr_get vars s h x); auto. rewrite e; simpl; auto.
+ apply (safeN_step _ _ _ _ H10).
+ specialize (H n'). rewrite semax'_unfold in H.
+ assert (necR n' (level w')). apply necR_trans with (level w); auto.
+ apply nec_nat. auto. apply necR_level'. auto.
+ specialize (H p G' _ H11 (pred_nec_hereditary _ _ _ H11 H1)).
+ specialize (H (locals2env s) w'').
+ spec H. omega.
+ specialize (H _ (necR_refl _)).
+ spec H.
+  rewrite andp_comm.
+ split. eapply pred_hereditary; eauto.
+ apply (pred_hereditary _ _ _ H7) in H5.
+ rewrite andp_assoc; split; [ |  apply H5].
+ hnf; auto.
+ apply H; auto.
+ apply (pred_nec_hereditary _ _ _ (rt_step _ _ _ _ H7)); auto. 
+ (* nonzero *)
+ subst.
+ assert (step p ((s,h), If x Then c1 Else c2) = Some ((s,h), c1)).
+ simpl. rewrite (eval_expr_get vars s h x); auto. simpl.  rewrite if_false; auto.
+ apply (safeN_step _ _ _ _ H10).
+ specialize (H n'). rewrite semax'_unfold in H.
+ assert (necR n' (level w')). apply necR_trans with (level w); auto.
+ apply nec_nat. auto. apply necR_level'. auto.
+ specialize (H p G' _ H11 (pred_nec_hereditary _ _ _ H11 H1)).
+ specialize (H (locals2env s) w'').
+ spec H. omega.
+ specialize (H _ (necR_refl _)).
+ spec H.
+ rewrite andp_comm.
+ split. eapply pred_hereditary; eauto.
+ apply (pred_hereditary _ _ _ H7) in H5.
+ rewrite andp_assoc; split; [ |  apply H5].
+ hnf; auto.
+ apply H; auto.
+ apply (pred_nec_hereditary _ _ _ (rt_step _ _ _ _ H7)); auto. 
+Qed.
+
+Lemma semax_load: forall x y z c vars G P,
+    expcheck vars y = true ->
+    semax (vs_add x vars) G P c -> 
+    semax vars G (fun s => ((mapsto (eval y s) z) * TT) && |> subst x z P s)
+               (Do x := Mem y ; c).
+Proof.
+ intros until P. intros TC [TC' ?].
+ split.
+ simpl; auto.
+ intro n.
+ rewrite semax'_unfold.
+ intros p G' n' ? ? s w ? w' ? [H5 H4].
+ destruct H5 as [[? HP] HG].
+ unfold subst in HP.
+ apply assert_safe0; intros w'' H7.
+ specialize (HP _ (t_step _ _ _ _ H7)).
+ intros s' h VC L ?. rewrite <- L in *; clear s L; rename s' into s.
+ generalize (age_level _ _ H7); intro. rewrite H8.
+ assert (step p ((s,h), Do x := Mem y; c) = Some ((table_set x z s, h), c)).
+ simpl. rewrite (eval_expr_get vars s h y); auto. simpl.
+ replace (heap_get h (eval y (locals2env s))) with (Some z).
+ auto.
+ symmetry.
+ apply H6. apply mapsto_e1; auto.
+ apply (safeN_step _ _ _ _ H9). clear H9.
+ specialize (H n'). rewrite semax'_unfold in H.
+ assert (necR n' (level w')). apply necR_trans with (level w); auto.
+ apply nec_nat. auto. apply necR_level'. auto.
+ specialize (H p G' _ H9 (pred_nec_hereditary _ _ _ H9 H1)).
+ specialize (H (locals2env (@table_set _ _ EqDec_var x z s)) w'').
+ spec H.    unfold R.rmap in *; omega. 
+ specialize (H _ (necR_refl _)).
+ spec H. split; [split|].
+  rewrite locals2env_table_set. eauto.
+  eapply pred_hereditary; eauto.
+  eapply pred_hereditary; eauto.
+ apply H; auto.
+ apply varcompat_add; auto.
+ eapply pred_hereditary; eauto.
+Qed.
+
+Lemma semax_store: forall x y v c vars G (P: assert),
+    expcheck vars x = true ->
+    expcheck vars y = true ->
+    semax vars G (fun s => mapsto (eval x s) (eval y s) * P s) c ->
+    semax vars G (fun s => mapsto (eval x s) v  * P s)  (Do Mem x  := y ; c).
+Proof.
+ intros until P; intros TCx TCy [TC ?].
+ split.
+ simpl; auto.
+ intro. rewrite semax'_unfold.
+ intros p G' n' ? ? s w ? w' ? [[H5 H6] H4].
+ apply assert_safe0; intros w'' ?.
+ intros s' h VC L ?. rewrite <- L in *; clear L s; rename s' into s.
+ generalize (age_level _ _ H7); intro. rewrite H9.
+ assert (step p ((s,h), Do Mem x := y; c) = Some ((s, heap_set (eval x (locals2env s)) (eval y (locals2env s)) h), c)).
+ simpl. rewrite (eval_expr_get vars s h y); auto. rewrite (eval_expr_get vars s h x); auto.
+ apply (safeN_step _ _ _ _ H10).
+ specialize (H n'). rewrite semax'_unfold in H.
+ assert (necR n' (level w')). apply necR_trans with (level w); auto.
+ apply nec_nat. auto. apply necR_level'. auto.
+ specialize (H p G' _ H11 (pred_nec_hereditary _ _ _ H11 H1)).
+ apply (pred_hereditary _ (level w') (level w'')) in H;
+   [ |  apply age_level in H7; rewrite H7; hnf; simpl; auto].
+ apply (pred_hereditary _ _ _ H7) in H5.
+ apply (pred_hereditary _ _ _ H7) in H6.
+ apply (pred_hereditary _ _ _ H7) in H4.
+ apply (pred_hereditary _ _ _ H7) in H8.
+ clear H1; pose (H1:=True). clear n H0. pose (H0:=True).
+ clear n' H2 H11. pose (H2:=True). pose (H11:=True).
+ simpl in H8.
+clear w' H7 H9 H3. 
+ pose (H7:=True); pose (H9:=True); pose (H3:=True).
+ clear H0 H1.
+ destruct H5 as [wa [wb [H0 [HP H1]]]].
+ pose (m' := singleton_rmap (eval x (locals2env s)) (eval y (locals2env s)) w'').
+ assert (joins m' wb).
+ apply resource_at_joins2. unfold m'.
+ rewrite singleton_rmap_level.
+ apply join_level in H0. destruct H0. auto.
+ unfold m'. intro i.
+ clear - HP H0.
+ apply (resource_at_join _ _ _ i) in H0.
+ specialize (HP i).
+ unfold singleton_rmap. rewrite resource_at_make_rmap.
+ destruct (eq_dec i (eval x (locals2env s))). subst; rewrite if_true in HP; auto.
+ exists (YES pfullshare (VAL (eval y (locals2env s))) NoneP).
+ rewrite HP in *. inv H0; try pfullshare_join. constructor.
+ rewrite if_false in HP by auto. 
+ exists (wb @ i). 
+ apply HP in H0. rewrite H0.
+ rewrite <- core_resource_at. apply core_unit.
+ destruct H5 as [ww H12].
+ replace (level w'') with (level ww) in H.
+ Focus 2.
+ transitivity (level wb).
+ apply join_level in H12. destruct H12 as [H12 H13]. symmetry ; apply H13.
+ apply join_level in H0; destruct H0; auto.
+ specialize (H (locals2env s) ww).
+ spec H. simpl. apply le_refl.
+ specialize (H _ (necR_refl _)).
+ spec H. rewrite andp_assoc. rewrite andp_comm.
+ clear - H4 H0 HP H12 H6 H1.
+ assert (app_pred ((mapsto (eval x (locals2env s)) v * TT) && (funassert G && funassert G')) w'').
+ split; auto. exists wa; exists wb; split3; auto. split; auto.
+ destruct H as [? _].
+ split.
+ apply join_comm in H0. apply join_comm in H12. apply join_core in H0. apply join_core in H12.
+ apply funassert_core in H6. apply funassert_core in H4. rewrite H12 in H0.
+ split; apply funassert_core; rewrite H0; auto.
+ destruct H as [wa' [wb' [? [? ?]]]].
+ assert (wa' = wa). eapply mapsto_uniq; eauto.
+ apply join_core in H0; apply join_core in H. rewrite H0; rewrite H. auto. 
+ subst wa'. generalize (join_canc (join_comm H0) (join_comm H)); intro; subst wb'.
+  generalize (singleton_rmap_mapsto (eval x (locals2env s)) (eval y (locals2env s)) w''); intro.
+ assert (app_pred (mapsto (eval x (locals2env s)) (eval y (locals2env s)) * (TT && (funassert G && funassert G'))) ww).
+ exists m'; exists wb; split3; auto.
+ split; auto.
+ apply join_comm in H0. apply join_comm in H12. apply join_core in H0. apply join_core in H12.
+  apply funassert_core in H6. apply funassert_core in H4.
+ split; apply funassert_core; rewrite H0; auto.
+ exists m'; exists wb; split3; auto.
+ replace (level w'') with (level ww).
+ Focus 2. simpl. transitivity (level wb).
+ clear - H12; apply join_level in H12; destruct H12; symmetry; apply H0.
+ clear - H0; apply join_level in H0; destruct H0; apply H0.
+ apply H; auto.
+ intros i v0. specialize (HP i).
+ simpl.
+ apply (resource_at_join _ _ _ i) in H12.
+ unfold m' in *; clear m'.
+ unfold singleton_rmap in H12.
+ rewrite resource_at_make_rmap in H12.
+ change AV.address with adr in H12.
+  specialize (H8 i v0). simpl in H8. 
+
+  destruct (eq_dec i (eval x (locals2env s))). 
+  subst. rewrite heap_gss.
+  apply join_unit2_e in H12. rewrite <- H12.
+  split; intro Hx; inv Hx; auto.
+  apply YES_join_full in H12; auto.
+  rewrite H12. apply NO_identity.
+  apply join_unit1_e in H12; [ | rewrite <- core_resource_at; apply core_identity].
+  rewrite heap_gso; auto. 
+ apply (resource_at_join _ _ _ i) in H0.
+ rewrite <- H12.
+ apply HP in H0. rewrite H0; auto.
+Qed.
+
+Lemma semax_pre: 
+  forall P P' vars G c, (forall s, P s |-- P' s) -> semax vars G P' c -> semax vars G P c.
+Proof.
+ intros. destruct H0 as [TC H0]; split; auto.
+ intro n; specialize (H0 n).
+ rewrite semax'_unfold in *.
+ intros p G'. specialize (H0 p G').
+ intros n' ? ?. specialize (H0 _ H1 H2).
+ intros s w ? ? ? ?. specialize (H0 s _ H3 _ H4).
+ apply H0.
+ destruct H5; split; auto. destruct H5;  split; auto. apply H; auto.
+Qed.
+
+
+Lemma semax_exp: forall {A} vars G (P: A -> assert) c,
+    typecheck vars c = true ->
+    (forall v:A, semax vars G (P v) c) ->
+    semax vars G (fun s => EX v:A, (P v s)) c.
+Proof.
+ intros ? ? ? ? ? TC ?.
+ split; auto. 
+ intro.
+ rewrite semax'_unfold.
+ intros p G'. intros n' ? ?.
+ intros s. intros ? ?. intros ? ?. intros [[[v ?] ?] ?].
+ specialize (H v). destruct H as [_ H].
+ rewrite semax'_unfold in H. eapply H; eauto. split; auto. split; auto.
+Qed.
+
+Lemma semax_exp': forall {A} (any: A) vars G (P: A -> assert) c,
+    (forall v:A, semax vars G (P v) c) ->
+    semax vars G (fun s => EX v:A, (P v s)) c.
+Proof.
+ intros ? ? ? ? ? ?.
+ split; auto. 
+ destruct (H any); auto.
+ intro.
+ rewrite semax'_unfold.
+ intros p G'. intros n' ? ?.
+ intros s. intros ? ?. intros ? ?. intros [[[v ?] ?] ?].
+ specialize (H v). destruct H as [_ H].
+ rewrite semax'_unfold in H. eapply H; eauto. split; auto. split; auto.
+Qed.
+
+Lemma semax_prop:
+  forall (R: Prop) vars G P c,
+      typecheck vars c = true ->
+      (R -> semax vars G P c) ->
+      semax vars G (fun s => !! R && P s) c.
+Proof.
+  intros R vars G P c TC ?. split; auto. intro n.  rewrite semax'_unfold. intros p G'.
+  intros n' ? ? b w ? w' ? [[[? ?] ?] ?].
+  destruct (H H4).
+  specialize (H9 n). rewrite semax'_unfold in H9.
+  eapply H9; eauto. split; auto. split; auto.
+Qed.
+
+Definition program_proved (p: program) :=
+   exists G, semax_func G p G  /\ table_get G 0 = Some (0::nil, fun s => allocpool (eval (Var 0) s)).
+
+Lemma semax_sound: 
+  forall p, program_proved p -> forall n, run p n <> None.
+Proof.
+  intros.
+  destruct H as [G [[? ?] ?]].
+  generalize (funassert_make_world p G n); intro.
+  destruct (semax_go nil G  (0::nil, fun s => allocpool (eval (Var 0) s))
+                (Const 0) (Const (boundary p) :: nil) (eq_refl _)) as [_ ?].
+  specialize (H3 n).
+  rewrite semax'_unfold in H3.
+  specialize (H3 p G _ (necR_refl _) (H0 _) (locals2env nil) 
+                    (make_world G (initial_heap p) n)).
+  spec H3. rewrite level_make_world. auto.
+  specialize (H3 _ (necR_refl _)).
+  spec H3.
+  split; auto.
+  split; auto.
+  split.
+  apply (funassert_e _ _ _ H1 _ H2).
+  unfold call.
+  Transparent arguments. unfold arguments. Opaque arguments.
+  simpl snd.
+  unfold locals2env, table_get. rewrite if_true; auto.
+  split. simpl; auto.
+  apply allocpool_make_world; auto.
+  hnf in H3.
+  specialize (H3 nil (initial_heap p)).
+  spec H3. intros i ?. inv H4.
+  spec H3. auto.
+  spec H3. apply cohere_make_world; auto.
+  unfold run; intro.
+  destruct H3 as [sk' ?].
+  rewrite level_make_world in H3. 
+ unfold locals,table, var,adr in H3,H4. rewrite H3 in H4; inv H4.
+Qed.
+
+End Semax.
