msl/subtypes_sl.v
@@ -200,3 +200,26 @@ intros w' ? ?. apply (H0 _ (necR_level' H2)).
 auto.
 Qed.
 Hint Resolve @subp_fash'.
+
+
+Lemma unfash_sepcon_distrib: 
+        forall {T}{agT: ageable T}{JoinT: Join T}{PermT: Perm_alg T}{SepT: Sep_alg T}{AgeT: Age_alg T} 
+           (P: pred nat) (Q R: pred T),
+               fash' P && (Q*R) = (fash' P && Q) * (fash' P && R).
+Proof.
+intros.
+apply pred_ext.
+intros w [? [w1 [w2 [? [? ?]]]]].
+exists w1; exists w2; repeat split; auto.
+apply join_level in H0. destruct H0.
+hnf in H|-*. congruence.
+apply join_level in H0. destruct H0.
+hnf in H|-*. congruence.
+intros w [w1 [w2 [? [[? ?] [? ?]]]]].
+split.
+apply join_level in H. destruct H.
+hnf in H0|-*. congruence.
+exists w1; exists w2; repeat split; auto.
+Qed.
+
+
